theories/examples/finelt/raw_validity.v
@@ -9,10 +9,13 @@ Set Implicit Arguments.
 Unset Strict Implicit.
 Unset Printing Implicit Defensive.
 
+Require Import smpl.Smpl.
+Require Import utils.all.
 
 Require Import syntax.syntax.
 Require Import syntax.typing.
 Require Import syntax.relations.
+
 
 
 Import SyntaxNotations.
@@ -52,456 +55,1473 @@ Proof.
   - rewrite (@IHM1 M3 M5) ; eauto.
 Qed.
 
+Lemma HeadRed_tpi_det (n:nat) (M : Tm n) A1 B1 A2 B2 : 
+  HeadRed M (Core.tpi A1 B1) -> HeadRed M (Core.tpi A2 B2) ->
+  A1 = A2 /\ B1 = B2.
+Proof.
+  move=> h1. move:A2 B2.
+  dependent induction h1.
+  all: move=> A2 B2 h2. 
+  - inversion h2; subst. done. inversion H.
+  - inversion h2; subst. inversion H.
+    specialize (IHh1 _ _ ltac:(reflexivity) A2 B2).
+    have EQ: e2 = e3. eapply HeadRed1_det; eauto.
+    subst.
+    eauto.
+Qed.
+
+Lemma HeadRed_tpi_eq {n}( A1 : Tm n) B1 A2 B2 :
+   HeadRed (Core.tpi A1 B1) (Core.tpi A2 B2) -> 
+   A1 = A2 /\ B1 = B2.
+Proof. 
+  move=> R1.
+  have R2: HeadRed (Core.tpi A1 B1) (Core.tpi A1 B1).
+  { eapply ms_refl. }
+  eapply HeadRed_tpi_det; eauto.
+Qed.
+
+Lemma typing_app_inv n (Γ : Ctx n) M N A : 
+ typing Γ (app M N) A -> 
+      exists A1 , exists A2, typing Γ M (tpi A1 A2) /\ typing Γ N A1 /\ conv Γ A2[N..] A tuniv.
+Proof. 
+  move=> h.
+  dependent induction h.
+  - specialize (IHh M N ltac:(eauto)).
+    destruct IHh as [A1 [A2 [TM [TN CC]]]].
+    exists A1. exists A2. repeat split; auto.
+    eapply c_trans; eauto.
+  - clear IHh1 IHh2 IHh3 IHh4.
+    exists A. exists B. repeat split; auto.
+    eapply c_refl; eauto.
+    eapply substitution_tm with (σ := N..) in h2. cbn in h2.
+    eapply h2.
+    eapply typing_subst_cons. asimpl. auto.
+    eapply typing_subst_id. eapply typing_ctx; eauto.
+    eapply typing_ctx; eauto.
+Qed.
+
+Lemma typing_abs_inv n (Γ : Ctx n) M A B: 
+ typing Γ (abs A M) B -> 
+      exists B2, typing (Γ ++ A) M B2 /\ conv Γ (tpi A B2) B tuniv.
+Proof. 
+  move=>h.
+  dependent induction h.
+  - specialize (IHh M A ltac:(eauto)).
+    destruct IHh as [B2 [TM CC]].
+    exists B2. repeat split; auto.
+    eapply c_trans; eauto.
+  - clear IHh1 IHh2 IHh3.
+    exists B. repeat split; auto.
+    eapply c_refl; eauto.
+    eapply t_tpi; eauto.
+Qed.
+
+
+Lemma HeadRed1_conv {n} Γ (M N : Tm n) A :
+  HeadRed1 M N -> typing Γ M A -> conv Γ M N A.
+Proof.
+  move=> h. induction h.
+  - move=> T.
+    destruct (typing_app_inv T) as [A1 [A2 [T1 [T3 C1]]]].
+    destruct (typing_abs_inv T1) as [B2 [T2 C2]].
+    eapply c_conv. 2: eassumption.
+    eapply c_beta; eauto.
+Abort.    
+
 Require Import findom.
 Require Import types.
-Require Import raw_semantics.
-Require Import typing_semantics.
-Require Import eval_substitution.
-
 
 Import Raw.
-    
 
-(* Logical relation, defined by induction on (semantic type) a.
-   We only need it for closed terms, so dropping the context and 
-   specializing M's scope to 0.
 
-   Swapped the order of arguments as we are pattern matching on 
-   u and a to define sets of term * type pairs.
-
-   As a is "more defined" this set becomes smaller. When we don't 
-   know anything, i.e. a is bot, then we have the total set.
-
-   If Val u a M A (h: wt u a) holds 
-   then we know that 
-     null |- M : A
- *)
-
+(*
 (* Inversion lemmas for wt *)
 Lemma wt_tpi_dom (a : elt) (g : list (elt * elt)) (j : nat):
-  wt (tpi a g) (tuniv j) ->
-  wt a (tuniv j).
+  wt (tpi a g) tuniv ->
+  wt a tuniv.
 move=>h. inversion h. done. Defined.
 Lemma wt_tpi_cod_key (a : elt) (g : list (elt * elt)) (j : nat):
-  wt (tpi a g) (tuniv j) ->
+  wt (tpi a g) tuniv ->
   (forall ui vi : elt, In (ui, vi) g -> wt ui a).
 move=>h. inversion h. done. Defined.
 Lemma wt_tpi_cod_elt (a : elt) (g : list (elt * elt)) (j : nat):
-  wt (tpi a g) (tuniv j) ->
-  (forall ui vi : elt, In (ui, vi) g -> wt vi (tuniv j)).
+  wt (tpi a g) tuniv ->
+  (forall ui vi : elt, In (ui, vi) g -> wt vi tuniv).
 move=>h. inversion h. done. Defined.
+*)
 
+(* This information is *not* availble from wt
+   TODO: update wt to include it
+   (And: if we want to have a recursively defined wt
+   we also need to update abs)
+ *)
+(*
+Lemma wt_abs_dom f a g : 
+  wt (abs f) (tpi a g) -> { i & wt a tuniv }.
+Proof.
+move=> h. inversion h. subst.
+inversion H4. subst. eexists. eauto.
+Qed.
+
+Lemma wt_abs_tpi f a g : 
+  wt (abs f) (tpi a g) -> { i &  wt (tpi a g) tuniv }.
+move=> h. inversion h. subst. eexists. eauto.
+Qed.
+*)
+(*
 Lemma wt_abs_key (a : elt) (f g : list (elt * elt)) :
   wt (abs f) (tpi a g) -> 
-  (forall ui vi w : elt, In (ui, vi) f -> app g ui = Some w -> wt ui a).
+  (forall ui vi : elt, In (ui, vi) f -> wt ui a).
 move=>h. inversion h. done. Defined.
 
 Lemma wt_abs_elt (a : elt) (f g : list (elt * elt)) :
   wt (abs f) (tpi a g) -> 
   (forall ui vi w : elt, In (ui, vi) f -> app g ui = Some w -> wt vi w).
 move=>h. inversion h. done. Defined.
+*)
 
-Lemma wt_succ_inv u:
-  wt (succ u) tnat -> wt u tnat.
-move=>h. inversion h. done. Defined.
 
-(* Unary logical relation *)
-Fixpoint Val (u : elt) (a: elt) 
-  (M : Tm 0) (A : Tm 0) (h : wt u a) { struct h } : Prop := 
-    typing ctx_empty M A 
-    /\ 
-      (match a return wt u _ -> Prop with 
+
+(* Logical relation, defined by recursion on the wt judgement for
+   semantic elements. i.e. on the derivation of `wt u a`.
+
+   The relation is parameterized by a typing context Γ : Ctx n.
+   Terms M, N, A live at scope n; substitutions B[N..] close one
+   variable, producing terms at scope n in the same context Γ.
+
+   This is a coinductive definition. As u is "more defined" the
+   set of syntactic terms in the relation becomes smaller.
+   To begin, when u is bot, it is the total set.
+
+*)
+
+
+(* This module defines various helper operations on the logical
+   relation. Each of these operations is parameterized by the
+   two main fixpoints (Val and EqVal) which are polymorphic in
+   the context size n and the typing context Γ.
+*)
+Module Rec.
+
+Record F := MkF {
+   Val   : forall {n} (Γ : Ctx n),
+              Tm n -> Tm n -> forall u a, wt u a -> Prop;
+   EqVal : forall {n} (Γ : Ctx n),
+              Tm n -> Tm n -> Tm n -> forall u a, wt u a -> Prop;
+}.
+
+Section Helpers.
+
+Variable 
+   Val   : forall {n} (Γ : Ctx n),
+              Tm n -> Tm n -> forall u a, wt u a -> Prop.
+Variable
+   EqVal : forall {n} (Γ : Ctx n),
+              Tm n -> Tm n -> Tm n -> forall u a, wt u a -> Prop.
+
+
+Definition  PiEdgeEq {n} (Γ : Ctx n)
+  (A : Tm n) (B : Tm (S n)) (b: elt) (f : list (elt * elt))
+  (h : wt (tpi b f) tuniv) :=
+  forall u v (Vu : valid u) 
+      (APP: app f u = Some v) (NB: ~ is_bot v) 
+      (N1 N2 : Tm n),
+      conv Γ N1 N2 A ->
+      (* take related arguments *)
+      EqVal Γ N1 N2 A (wt_tpi_inv1 h Vu APP NB) ->
+      (* to related results *)
+      EqVal Γ B[N1..] B[N2..] Core.tuniv (wt_tpi_inv2 h Vu APP NB).
+
+Definition PiAppVal {n} (Γ : Ctx n)
+  (M : Tm n) (A0 : Tm n) (B0 : Tm (S n)) b f g
+  (h : wt (abs f) (tpi b g)) : Prop :=
+  forall u v t (Vu : valid u) 
+  (APP: app f u = Some v) (NB: ~ is_bot v) 
+  (APPg : app g u = Some t)
+  (P : Tm n), typing Γ P A0 -> 
+              Val  Γ P A0 (wt_abs_inv1 h Vu APP NB) -> 
+              Val  Γ (Core.app M P) B0[P..] 
+                  (wt_abs_inv2 h Vu APP NB APPg). 
+
+Definition PiAppEq {n} (Γ : Ctx n)
+  (M : Tm n) (A0 : Tm n) (B0 : Tm (S n)) b f g
+  (h : wt (abs f) (tpi b g))  := 
+  forall u v t (Vu : valid u) 
+    (APP: app f u = Some v) (NB: ~ is_bot v) 
+    (APPg : app g u = Some t)
+    (N1 N2 : Tm n),
+    conv Γ N1 N2 A0 ->
+    EqVal  Γ N1 N2 A0 (wt_abs_inv1 h Vu APP NB) ->
+    EqVal  Γ (Core.app M N1) (Core.app M N2) B0[N1..] 
+          (wt_abs_inv2 h Vu APP NB APPg).
+    
+Definition PiAppEqVal {n} (Γ : Ctx n)
+  (M N : Tm n) (A0 : Tm n) (B0 : Tm (S n)) b f g
+  (h : wt (abs f) (tpi b g)) :=
+  forall  u v t (Vu : valid u) 
+  (APP: app f u = Some v) (NB: ~ is_bot v) 
+  (APPg : app g u = Some t) (P : Tm n),
+        typing Γ P A0 ->
+        Val  Γ P A0 (wt_abs_inv1 h Vu APP NB) ->
+        EqVal  Γ (Core.app M P) (Core.app N P) B0[P..]
+          (wt_abs_inv2 h Vu APP NB APPg).
+
+Definition ValPi {n} (Γ : Ctx n)
+  (M : Tm n) (A : Tm n) g b f (h : wt (abs g) (tpi b f)):=
+  exists A0, exists B0, HeadRed A (Core.tpi A0 B0)
+  /\ PiAppVal Γ M A0 B0 h.
+
+Definition EqValPi {n} (Γ : Ctx n)
+  (M : Tm n) (N: Tm n) (A : Tm n) g b f 
+  (h : wt (abs g) (tpi b f)) :=
+  exists A0, exists B0, HeadRed A (Core.tpi A0 B0)
+  /\ PiAppEqVal Γ M N A0 B0 h.
+
+Fixpoint ValTy {n} (Γ : Ctx n)
+  (M : Tm n) u (h : wt u tuniv) {struct h} : Prop  :=
+
+  let PiEdgeVal {n} (Γ : Ctx n)
+        (A : Tm n) (B : Tm (S n)) (b: elt) (f : list (elt * elt))
+        (h : wt (tpi b f) tuniv) : Prop := 
+    forall u v (Vu : valid u) 
+        (APP: app f u = Some v) (NB: ~ is_bot v) (WTu : wt u b)
+        (N : Tm n), typing Γ N A ->
+                    (* take related arguments *)
+                    Val  Γ N A (wt_tpi_inv1 h Vu APP NB) ->
+                    (* to related results *)
+                    ValTy Γ B[N..] (wt_tpi_inv2 h Vu APP NB)
+  in
+
+  (match u return wt _ tuniv ->  Prop with
+  | tpi b g =>
+      fun (h : wt (tpi b g) tuniv) =>
+        (* ValTyPi M tuniv *)
+        (* M reduces to a pi type *)
+        exists A B, HeadRed M (Core.tpi A B)
+
+               (* the syntactic pi-type is well-typed *)              
+               /\ typing Γ A Core.tuniv
+               /\ typing (Γ ++ A) B Core.tuniv
+
+               (* the semantic pi-type is valid *)
+               /\ valid (tpi b g)
+
+               (* domain (b) is in the relation *)
+               /\ Val  Γ A Core.tuniv (wt_tpi_dom h)
+                                          
+               /\ PiEdgeVal Γ A B b g h 
+               /\ PiEdgeEq Γ A B h
+
+  | tnat => fun h1 => True
+  | tuniv => fun h1  => True
+  | _ => fun h1  => True
+  end) h.
+
+
+Fixpoint EqValTy {n} (Γ : Ctx n) M N (a : elt) (h : wt a tuniv) {struct h} :  Prop :=
+  let PiEdgeEqTy {n} (Γ : Ctx n) 
+  (A : Tm n) (B B' : Tm (S n)) b f (h : wt (tpi b f) tuniv)  := 
+    forall u v (Vu : valid u) 
+      (APP: app f u = Some v) (NB: ~ is_bot v) 
+      (P : Tm n),
+          typing Γ P A ->
+          (* take related arguments *)
+          Val  Γ P A (wt_tpi_inv1 h Vu APP NB) ->
+          (* to related results *)
+          EqValTy Γ B[P..] B'[P..] (wt_tpi_inv2 h Vu APP NB)
+  in 
+  (match a return wt _ tuniv ->  Prop with
+  | tpi b f =>
+      fun (h : wt (tpi b f) tuniv)  =>
+        ValTy Γ M h  /\ ValTy Γ N h /\
+        (* EqValTyPi Val EqVal EqValTy M N h *)
+             (* both reduce to pi types *)
+             exists A B, HeadRed M (Core.tpi A B)
+             /\ exists A' B', HeadRed N (Core.tpi A' B')
+             (* ... that are convertible *)
+             /\ conv Γ A A' Core.tuniv 
+             /\ conv (Γ ++ A) B B' Core.tuniv 
+             /\ valid (tpi b f)
+             (* ... and the domain is in the relation *)
+             /\ EqVal  Γ A A' Core.tuniv  (wt_tpi_dom h) 
+             /\ PiEdgeEqTy Γ A B B' _ _ h
+  | _ => fun h => True
+  end) h.
+
+End Helpers.
+End Rec.
+
+
+Fixpoint Val {n} (Γ : Ctx n)
+  (M : Tm n) (A : Tm n) (u : elt) (a: elt) (h : wt u a)  
+  { struct h } : Prop :=
+      (match a return wt u _ -> Prop with
 
       | bot => fun h => True
-                
-      | tuniv i => fun h =>
-          HeadRed A (Core.tuniv i) /\
-          (* This is ValTy *)
-          (match u return wt _ (tuniv i) -> Prop with 
-            | bot => fun h => True 
-               
-            | tpi b g => fun (h : wt (tpi b g) (tuniv i)) =>
-              exists A1 B1, HeadRed M (Core.tpi A1 B1) 
-              /\ @Val b (tuniv i) A1 (Core.tuniv i) (wt_tpi_dom h)
-              /\ forall u v (IN : In (u,v) g) (M1 : Tm 0),
-                  (* take related arguments *)
-                  @Val u b M1 A1 (wt_tpi_cod_key h IN) ->
-                  (* to related results *)
-                  @Val v (tuniv i) B1[M1..] (Core.tuniv i)
-                       (wt_tpi_cod_elt h IN)
 
-            | tuniv j => fun h => 
-              HeadRed M (Core.tuniv j)  
+      | tuniv => fun (h : wt u tuniv) =>
+          Rec.ValTy (@Val) (@EqVal) Γ M h 
 
-            | tnat => fun h =>
-              HeadRed M (Core.tnat)  
+      | tpi b f => fun h  =>
+           (match u return wt _ (tpi b f) ->  Prop with
 
-            | _ => fun h => False 
-            end) h
+            | abs g => fun (h : wt (abs g) (tpi b f)) =>
+                        Rec.ValTy (@Val) (@EqVal) Γ A (wt_abs_ty h)
+                      /\ Rec.ValPi (@Val) Γ M A h 
 
-      | tpi b f => fun h => 
-           exists A1 B1, HeadRed A (Core.tpi A1 B1) /\
-           (match u return wt _ (tpi b f) -> Prop with
-           | bot => fun h => True 
-           | abs g => fun (h : wt (abs g) (tpi b f)) => 
-             exists M1, HeadRed M (Core.abs A1 M1) 
-                 /\ forall u v (IN: In (u,v) g) w 
-                     (APPf : app f u = Some w) (N : Tm 0), 
-                 (* take related arguments *)
-                 @Val u b N A1 (wt_abs_key h IN APPf) ->
-                 (* to related results *)
-                 @Val v w M1[N..] B1[N..]
-                       (wt_abs_elt h IN APPf)
-
-           | _ => fun h => False 
-            end) h
+            | _ => fun h  => True
+            end) h 
 
       | tnat => fun h =>
-          HeadRed A (Core.tnat) /\
-          (match u return wt _ tnat -> Prop with 
-               | zero => fun h => 
+          (match u return wt _ tnat -> Prop with
+               | zero => fun h  =>
                  HeadRed M (Core.zero)
-               | succ v => fun (h : wt (succ v) tnat) => 
+               | succ v => fun (h : wt (succ v) tnat)  =>
                  exists M1, HeadRed M (Core.succ M1)
-                 /\ @Val v tnat M1 Core.tnat (wt_succ_inv h)
+                 /\ Val Γ M1 Core.tnat (wt_succ_inv h) 
                | _ =>  fun h => True
                end) h
-      | _ => fun h => True
-    end) h.
-
+      | _ => fun h  => True
+       end) h 
 (* Binary logical relation *)
-Fixpoint EqVal (u : elt) (a: elt) 
-  (M : Tm 0) (N : Tm 0) (A : Tm 0) (h : wt u a) { struct h } : Prop := 
-    conv ctx_empty M N A 
-    /\ 
-      (match a return wt u _ -> Prop with 
+with EqVal {n} (Γ : Ctx n)
+  (M : Tm n) (N : Tm n) (A : Tm n) (u : elt) (a: elt) (h : wt u a) 
+  { struct h } : Prop :=
+       
+     (match a return wt u _ -> Prop with
 
       | bot => fun h => True
-                
-      | tuniv i => fun h =>
-          HeadRed A (Core.tuniv i) /\
-          (* This is ValTy *)
-          (match u return wt _ (tuniv i) -> Prop with 
-            | bot => fun h => True 
-               
-            | tpi b g => fun (h : wt (tpi b g) (tuniv i)) =>
-              exists A1 B1, HeadRed M (Core.tpi A1 B1) 
-              /\ exists A2 B2, HeadRed N (Core.tpi A2 B2)
-              /\ @EqVal b (tuniv i) A1 A2 (Core.tuniv i) (wt_tpi_dom h)
-              /\ forall u v (IN : In (u,v) g) (N1 N2 : Tm 0),
-                  (* take related arguments *)
-                  @EqVal u b N1 N2 A1 (wt_tpi_cod_key h IN) ->
-                  (* to related results *)
-                  @EqVal v (tuniv i) B1[N1..] B2[N2..] (Core.tuniv i)
-                       (wt_tpi_cod_elt h IN)
 
-            | tuniv j => fun h => 
-              HeadRed M (Core.tuniv j)  
+      | tuniv => fun (h : wt u tuniv) =>
 
-            | tnat => fun h =>
-              HeadRed M (Core.tnat)  
+            Rec.ValTy (@Val) (@EqVal) Γ M h
+          /\ Rec.ValTy (@Val) (@EqVal) Γ N h
+          /\ Rec.EqValTy (@Val) (@EqVal) Γ M N h 
 
-            | _ => fun h => False 
-            end) h
-
-      | tpi b f => fun h => 
-           exists A1 B1, HeadRed A (Core.tpi A1 B1) /\
+      | tpi b f => fun h =>
            (match u return wt _ (tpi b f) -> Prop with
-           | bot => fun h => True 
-           | abs g => fun (h : wt (abs g) (tpi b f)) => 
-             exists M1, HeadRed M (Core.abs A1 M1) 
-             /\ exists N1, HeadRed N (Core.abs A1 N1)
-             /\ forall u v (IN: In (u,v) g) w 
-                     (APPf : app f u = Some w) (M2 N2 : Tm 0), 
-                 (* take related arguments *)
-                 @EqVal u b M2 N2 A1 (wt_abs_key h IN APPf) ->
-                 (* to related results *)
-                 @EqVal v w M1[M2..] N1[N2..] B1[M2..]
-                       (wt_abs_elt h IN APPf)
+           | bot => fun h => True
+           | abs g => fun (h : wt (abs g) (tpi b f)) =>
+               Rec.ValTy (@Val) (@EqVal) Γ A (wt_abs_ty h)
+             /\ Rec.ValPi (@Val)  Γ M A h
+             /\ Rec.ValPi (@Val)  Γ N A h
+             /\ Rec.EqValPi (@Val) (@EqVal) Γ M N A h
 
-           | _ => fun h => False 
+           | _ => fun h => True
             end) h
 
       | tnat => fun h =>
-          HeadRed A (Core.tnat) /\
-          (match u return wt _ tnat -> Prop with 
-               | zero => fun h => 
+          (match u return wt _ tnat -> Prop with
+               | zero => fun h =>
                  HeadRed M Core.zero
                  /\ HeadRed N Core.zero
-               | succ v => fun (h : wt (succ v) tnat) => 
+               | succ v => fun (h : wt (succ v) tnat) =>
                  exists M1, HeadRed M (Core.succ M1)
                  /\ exists N1, HeadRed N (Core.succ N1)
-                 /\ @EqVal v tnat M1 N1 Core.tnat (wt_succ_inv h)
+                 /\ EqVal Γ M1 N1 Core.tnat (wt_succ_inv h)
                | _ =>  fun h => True
                end) h
       | _ => fun h => True
     end) h.
 
 
-(* All terms in the relation have the right type. *)
-Fixpoint Val_typing (u : elt) (a: elt) 
-  (M : Tm 0) (A : Tm 0) (h : wt u a) :
-  Val M A h -> typing ctx_empty M A.
+
+Arguments Val : clear implicits.
+Arguments EqVal : clear implicits.
+
+Notation PiAppVal := (@Rec.PiAppVal Val).
+Notation ValTy    := (@Rec.ValTy Val EqVal).
+Notation EqValTy  := (@Rec.EqValTy Val EqVal).
+Notation ValPi    := (@Rec.ValPi Val).
+Notation EqValPi  := (@Rec.EqValPi Val EqVal).
+Notation PiEdgeEq := (@Rec.PiEdgeEq EqVal).
+Notation PiAppEqVal := (@Rec.PiAppEqVal Val EqVal).
+
+Arguments Val {_} _ _ _ {_}{_}.
+Arguments EqVal {_} _ _ _ _ {_}{_}.
+
+
+(* All terms in the relation have the right syntactic type.
+ NOT TRUE*)
+Fixpoint Val_typing {n} (Γ : Ctx n) (u : elt) (a: elt)
+  (M : Tm n) (A : Tm n) (h : wt u a) :
+  Val Γ M A h -> typing Γ M A.
 Proof.
   dependent destruction h.
-  all: move=> [h1 h2].
-  all: done.
-Qed.
+  all: move=> h1.
+  all: cbn in h1.
+  - destruct a; try done.
+Abort.
 
-
-
-(* Fundamental theorem for the logical relation 
-   
-   We want to show that well-typed terms are in the 
-   relation.
-
-   - If Γ |- M : A (typing) then
-
-
-     if Γ |= ρ ~ σ  (ValSub)
-
-          and  Γ |- σ  (typing_subst ctx_empty)
-
-          and  Γ |= ρ  (fits)   
-
-
-     for all u, a, such that h ∈ u : a   (wt)
-
-        where [[M]]ρ = u  and [[A]]ρ = a  (EvalRel)
-
-     we have
-
-        Val u a M[σ] A[σ] h
-
-   - If Γ |- M = N : A  (conv) 
-
-     and  Γ |- σ1  Γ |- σ2 (typing_subst ctx_empty)
-
-     and  Γ |= ρ  (fits)   
-
-     and [[M]]ρ = u and [[N]]ρ = u and [[A]]ρ = a  (EvalRel)
- 
-     and h ∈ u : a   (wt)
-
-     and Γ |= ρ ~ σ1 == σ2   (EqValSub)
-
-     then
-
-     EqVal u a M[σ1] N[σ2] A[σ] h
+(*
+Lemma EqVal_tpi n (Γ:Ctx n) M N A f g a i u b (w : wt_pi_fun g a i) (h : wt a tuniv) (V : valid (tpi a g)) :
+  (EqVal Γ M N A (wt_tpi w h V : wt u b)) =
+      (match h return wt _ (tpi a g) -> Prop with
+           | bot => fun h => True
+           | abs g => fun (h : wt (abs f) (tpi a g)) =>
+              match h with
+              | wt_abs WTf Vf (wt_tpi _ WTa _) =>
+                  Rec.ValTy Rec Γ A WTa
+              | _ => True
+              end
+             /\ Rec.ValPi Rec Γ M A h
+             /\ Rec.ValPi Rec Γ N A h
+             /\ Rec.EqValPi Rec Γ M N A h
+       end).
 *)
 
 
-(* A closing substitution: σ *)
-Definition Sub m := fin m -> Tm O.
 
-(* A valid closing substitution σ maps every term to one that 
-   can be interpreted. *) 
-Definition ValSub {g} (Γ : Ctx g) (ρ : Env g) (σ : Sub g)  : Prop := 
-  forall i,
-  forall u, valid u -> le u (ρ i) ->
-    forall a, EvalRel (lookup i Γ) ρ a ->
-    forall (h : wt u a), 
-      Val (σ i) (lookup i Γ)[σ] h. 
+(* ============================================================
+   Val2-Bot, EqVal2-Bot: at u = bot, both relations are True.
+   ============================================================ *)
 
-
-Lemma ValSub_empty : ValSub ctx_empty null null.
-unfold ValSub. done. Qed.
-
-Lemma ValSub_cons {g} (Γ : Ctx g) (ρ : Env g) (σ : Sub g) A v (M : Tm 0): 
-    (forall u, valid u -> le u v -> forall a (h : wt u a),
-    EvalRel A ρ a -> 
-    Val M A[σ] h) -> 
-    ValSub Γ ρ σ -> 
-    ValSub (Γ ++ A) (v .: ρ) (M .: σ). 
-Proof.
-  intros hyp0 VS.
-  unfold ValSub in *.
-  move=> i u0 Vu0 Le0 a0 E0 WT0.
-  destruct i as [i|].
-  - (* succ case *) 
-    cbn in *. asimpl.
-    eapply VS; eauto.
-    eapply EvalRel_unwk in E0; auto.
-  - (* zero case *)
-    cbn in *. asimpl.
-    eapply EvalRel_unwk in E0; auto.
-Qed.    
-
-Definition EqValSub {g} (Γ : Ctx g) (ρ : Env g) 
-  (σ1 : Sub g) (σ2 : Sub g)  : Prop := 
-  forall i, 
-  forall u, valid u -> le u (ρ i) ->
-    forall a, EvalRel (lookup i Γ) ρ a ->
-    forall (h : wt u a), 
-      EqVal (σ1 i) (σ2 i) (lookup i Γ)[σ1] h. 
-
-Lemma EqValSub_empty : EqValSub ctx_empty null null null.
-unfold EqValSub. done. Qed.
-
-Lemma EqValSub_cons {g} (Γ : Ctx g) (ρ : Env g) 
-  (σ1 σ2 : Sub g) A v (M1 M2 : Tm 0): 
-    (forall u, valid u -> le u v -> forall a (h : wt u a),
-    EvalRel A ρ a -> 
-    EqVal M1 M2 A[σ1] h) -> 
-    EqValSub Γ ρ σ1 σ2 -> 
-    EqValSub (Γ ++ A) (v .: ρ) (M1 .: σ1) (M2 .: σ2). 
-Proof.
-  intros hyp0 VS.
-  unfold ValSub in *.
-  move=> i u0 Vu0 Le0 a0 E0 WT0.
-  destruct i as [i|].
-  - (* succ case *) 
-    cbn in *. asimpl.
-    eapply VS; eauto.
-    eapply EvalRel_unwk in E0; auto.
-  - (* zero case *)
-    cbn in *. asimpl.
-    eapply EvalRel_unwk in E0; auto.
-Qed.    
-
-Definition semantic_typing {n} (Γ : Ctx n) (M : Tm n) (A : Tm n) :=
-  forall ρ σ (TS : typing_subst ctx_empty σ Γ) (F : fits Γ ρ) 
-    (VS : ValSub Γ ρ σ), 
-  forall u a (WT : wt u a), 
-    EvalRel M ρ u -> 
-    EvalRel A ρ a -> 
-    Val M[σ] A[σ] WT.
-Definition semantic_conv {n} (Γ : Ctx n) (M N: Tm n) (A : Tm n) :=
-  forall ρ σ (TS : typing_subst ctx_empty σ Γ) (F : fits Γ ρ)
-    (VS : ValSub Γ ρ σ), 
-  forall u a (WT : wt u a), 
-    EvalRel M ρ u -> 
-    EvalRel A ρ a -> 
-    EqVal M[σ] N[σ] A[σ] WT. 
-Definition semantic_conv2 {n} (Γ : Ctx n) (M N: Tm n) (A : Tm n) :=
-  forall ρ σ1 σ2 (TS1 : typing_subst ctx_empty σ1 Γ) 
-            (TS2 : typing_subst ctx_empty σ2 Γ)
-    (F : fits Γ ρ)
-    (VS : EqValSub Γ ρ σ1 σ2), 
-  forall u a (WT : wt u a), 
-    EvalRel M ρ u -> 
-    EvalRel A ρ a -> 
-    EqVal M[σ1] N[σ2] A[σ1] WT. 
-
-Notation "Γ ⊨ M ∈ A" := (semantic_typing Γ M A) (at level 70).
-Notation "Γ ⊨ M ≡ N ∈ A" := (semantic_conv Γ M N A) (at level 70).
-
-(* ------------------ semantic typing rules ----------- *)
-
-Section SemanticTyping.
-
-Variable (n:nat) (Γ : Ctx n).
-
-Lemma st_var (x : fin n) : 
-  ctx Γ -> 
-(* ------------------------- *)
-  Γ ⊨ var x ∈ lookup x Γ.
-Proof.
-  move=> h. 
-  move=> ρ σ TS FR VS u1 a1 WT1 Ex ER.
-  cbn in *. move: Ex => [Vu1 Le1].
-  specialize (VS x).
-  eapply VS; eauto.
+Lemma Val_Bot {n} (Γ : Ctx n) (M A : Tm n) a (h : wt bot a) : Val Γ M A h.
+Proof. dependent destruction h.
+       destruct a eqn:EQa; try done.
 Qed.
 
-Lemma st_conv M A B i : 
-  Γ ⊨ M ∈ A -> 
-  Γ ⊨ A ≡ B ∈ Core.tuniv i ->
-(* ------------------------- *)
-  Γ ⊨ M ∈ B.
+Lemma EqVal_Bot {n} (Γ : Ctx n) (M N A : Tm n) a (h : wt bot a) :
+  EqVal Γ M N A h.
 Proof.
-  move=> h1 h2. 
-  move=> ρ σ TS FR VS u1 a1 WT1 Ex ER.
-  specialize (h1 ρ σ TS FR VS).
-  specialize (h2 ρ σ TS FR VS).
-Admitted.  
+dependent destruction h.
+       destruct a eqn:EQa; try done.
+Qed.
 
-Lemma st_abs A B M i : 
-  Γ ⊨ A ∈ Core.tuniv i -> 
-  Γ ++ A ⊨ B ∈ Core.tuniv i -> 
-  Γ ++ A ⊨ M ∈ B ->
-(* ------------------------- *)
-  Γ ⊨ Core.abs A M ∈ Core.tpi A B.
+
+(* ============================================================
+   Val <-> ValTy  and  EqVal <-> EqValTy
+   ============================================================ *)
+
+Lemma EqValTy_EqVal {n} (Γ : Ctx n) (A B : Tm n) a (h : wt a tuniv):
+  EqValTy Γ A B h ->
+  EqVal Γ A B Core.tuniv h.
+Proof.
+  dependent destruction h; try done.
+  all: cbn.
+  all: move=> [hA [hB h1]].
+  all: eauto.
+Qed.
+
+Lemma EqVal_EqValTy {n} (Γ : Ctx n) (A B C : Tm n) a (h : wt a tuniv):
+  EqVal Γ A B C h ->
+  EqValTy Γ A B h.
+Proof.
+  dependent destruction h; try done.
+  all: cbn in *.
+  all: eauto.
+Qed.
+
+Lemma ValTy_Val {n} (Γ : Ctx n) (A : Tm n) a (h : wt a tuniv):
+  ValTy Γ A h ->
+  Val Γ A Core.tuniv h.
+Proof.
+  dependent destruction h; try done.
+Qed.
+
+Lemma Val_ValTy {n} (Γ : Ctx n) (A : Tm n) a (h : wt a tuniv):
+  Val Γ A Core.tuniv h ->
+  ValTy Γ A h.
+Proof.
+  dependent destruction h; try done.
+Qed.
+
+                                  
+
+
+(* ============================================================
+   Diagonal embedding
+   Val <-> EqVal  and  ValTy → EqValTy
+   ============================================================ *)
+
+
+Fixpoint Val_EqVal {n} (Γ : Ctx n) (M A : Tm n) u a (h : wt u a) {struct h} :
+  Val Γ M A h -> EqVal Γ M M A h.
+Proof.
++ dependent destruction h.
+  all: cbn.
+  all: eauto.
+  - destruct a; try done.
+  - 
+    move=> [M1 [h1 V1]].
+    exists M1. split; auto.
+    exists M1. split; auto.
+  - (* tpi *) 
+    move=>h1.
+    repeat split; eauto.
+    clear A.
+    destruct h1 as (A & B & HR &  TA & TB & VPi & ValA & PEV & PEE).
+    exists A, B. split; auto.
+    exists A, B. split; auto.
+    repeat split; auto.
+    eapply c_refl; eauto.
+    eapply c_refl; eauto. 
+    move=> u v Vu APP NB P TP VA.
+    unfold PiEdgeEq in PEE.
+    specialize (PEV u v Vu APP NB).
+    specialize (PEE u v Vu APP NB).
+    eapply EqVal_EqValTy.
+    eapply PEE.
+    eapply c_refl; eauto.
+    cbn.
+    eapply Val_EqVal. eapply VA.
+  - (* abs *)
+    move=> [HR PAV].
+    inversion h. subst.
+    repeat split; eauto.
+    unfold Rec.ValPi in PAV.
+    destruct PAV as [A0 [B0 [R1 PAV]]].
+    unfold EqValPi.
+    exists A0, B0. split; eauto.
+    unfold PiAppEqVal.
+    unfold PiAppVal in PAV.
+    move=> u v t Vu APP NB APPg P TP VP.
+    specialize (PAV u v t Vu APP NB APPg P TP VP).
+    eapply Val_EqVal.
+    cbn. cbn in PAV.
+    auto.
+Defined.
+
+
+(* ValTy2-to-EqValTy2 *)
+Lemma ValTy_EqValTy {n} (Γ : Ctx n) (M : Tm n) u (h : wt u tuniv) :
+  ValTy Γ M h -> EqValTy Γ M M h.
+Proof.
+  intros VT.
+  eapply EqVal_EqValTy.
+  eapply Val_EqVal.
+  eapply ValTy_Val.
+  auto.
+Qed.
+
+
+(* ============================================================
+   Level 1 — projecting first and second parts of EqVal
+   EqVal_Val1, EqVal_Val2
+   ============================================================ *)
+
+
+Fixpoint EqVal_Val1 {n} (Γ : Ctx n) (M N A : Tm n) u a (h : wt u a) {struct h} :
+  EqVal Γ M N A h -> Val Γ M A h.
+Proof.
+  dependent destruction h.
+  all: cbn.
+  all: eauto.
+  (* 2 nontrivial goals *)
+  - destruct a; try done.
+  - move=> [M1 [h1 [N1 [h2 V1]]]].
+    exists M1. split; auto.
+    eauto.
+Qed.
+
+
+Fixpoint EqVal_Val2 {n} (Γ : Ctx n) (M N A : Tm n) u a (h : wt u a) {struct h} :
+  EqVal Γ M N A h -> Val Γ N A h.
+Proof.
+  dependent destruction h.
+  all: cbn.
+  all: eauto.
+  (* 2 nontrivial goals *)
+  - destruct a; try done.
+  - move=> [M1 [h1 [N1 [h2 V1]]]].
+    exists N1. split; auto.
+    eauto.
+Qed.
+
+(* ============================================================
+   Level 1a — 
+   Head reduction/expansion
+   ============================================================ *)
+
+Lemma HeadRed_expand {n} (M M' : Tm n) A B :
+  HeadRed1 M M' ->
+  HeadRed M'  (Core.tpi A B) ->
+  HeadRed M (Core.tpi A B).
+Proof.
+  move=> R HR.
+  eapply ms_trans; eauto.
+Qed.
+
+Lemma HeadRed_contract {n} (M M' : Tm n) A B :
+  HeadRed1 M M' ->
+  HeadRed M  (Core.tpi A B) ->
+  HeadRed M' (Core.tpi A B).
+Proof.
 Admitted.
 
-Lemma st_app A B N M i : 
-(*  Γ |- A ∈ Core.tuniv i -> 
-  Γ ++ A |- B ∈ Core.tuniv i -> 
-  Γ |- M ∈ (Core.tpi A B) -> 
-  Γ |- N ∈ A  ->  *)
-  Γ ⊨ A ∈ Core.tuniv i -> 
-  Γ ++ A ⊨ B ∈ Core.tuniv i -> 
-  Γ ⊨ M ∈ (Core.tpi A B) -> 
-  Γ ⊨ N ∈ A  -> 
-(* ------------------------ *)
-  Γ ⊨ Core.app M N ∈ B[N..].
-Proof.
-  move=> h1 h2 h3 h4 (* h1' h2' h3' h4' *). 
-  move=> ρ σ TS FR VS u1 a1 WT1 Ex ER.
-  specialize (h1 ρ σ TS FR VS).
-(*   specialize (h2 ρ σ TS FR VS). *)
-  specialize (h3 ρ σ TS FR VS).
-  specialize (h4 ρ σ TS FR VS).
-  cbn.
-  cbn in Ex.
-  destruct (is_bot u1) eqn:HB. 
-  - (* EvalRel (app M N) is bot *)
-    admit.
-  - (* EvalRel (app M N) comes from an application *)
-    move: Ex => [u0 [EM EN]].    
-    move: (h3 (u0 ↦ u1)) => h3'.
-    (* we need to get a type for (u0 |-> u1). *)
-Admitted.
- 
+Lemma ValTy_HeadRed1_expand {n} (Γ : Ctx n) (M M' : Tm n) u (h : wt u tuniv) :
+  HeadRed1 M' M -> ValTy Γ M h -> ValTy Γ M' h.
+Proof. 
+  move=> R.
+  dependent destruction h.
+  all: cbn; try done.
+  move=> [A0 [B0 [R0 [TA0 [TB0 [Vpi [VA [PEV PEE]]]]]]]].
+  exists A0. exists B0.
+  repeat split; eauto.
+  eapply HeadRed_expand; eauto.
+Qed.
 
-End SemanticTyping.
-
-
- 
-(* 
-  -- Main bundled adequacy theorem
-  adequacySub2 : {h g : Nat} {H : Ctx h} {G : Ctx g}
-    {M A : Expr g} ->
-    HasType G M A ->       (* syntax.typing *)
-    (sigma : Sub h g) -> 
-    (rho : EnvApprox g) ->  (* Env *)
-    CoherentEnv rho ->  (* valid_env *)
-    ValidSub2 H G sigma rho -> 
-    Fits G rho ->
-    WtSub H G sigma -> WfCtx H ->
-    (u : FinEl) -> EvalRel M rho u ->
-    (a : FinEl) -> EvalRel A rho a -> FinMem u a ->
-    Val2 H (substExpr sigma M) (substExpr sigma A) u a
-
-  -- Bundled adequacy for conversion
-  adequacyEqSub2 : {h g : Nat} {H : Ctx h} {G : Ctx g}
-    {M N A : Expr g} ->
-    ConvTm G M N A ->
-    (sigma : Sub h g) -> (rho : EnvApprox g) ->
-    CoherentEnv rho -> ValidSub2 H G sigma rho -> Fits G rho ->
-    WtSub H G sigma -> WfCtx H ->
-    (u : FinEl) -> EvalRel M rho u ->
-    (a : FinEl) -> EvalRel A rho a -> FinMem u a ->
-    EqVal2 H (substExpr sigma M) (substExpr sigma N) (substExpr sigma A) u a
-
-  -- Two-substitution adequacy
-  adequacyConvSub2 : {h g : Nat} {H : Ctx h} {G : Ctx g}
-    {M A : Expr g} ->
-    HasType G M A ->
-    (sigma sigma' : Sub h g) -> (rho : EnvApprox g) ->
-    CoherentEnv rho ->
-    ValidSub2 H G sigma rho -> ValidSub2 H G sigma' rho ->
-    ValidConvSub2 H G sigma sigma' rho ->
-    Fits G rho ->
-    WtSub H G sigma -> WtSub H G sigma' ->
-    WtConvSub H G sigma sigma' ->
-    WfCtx H ->
-    (u : FinEl) -> EvalRel M rho u ->
-    (a : FinEl) -> EvalRel A rho a -> FinMem u a ->
-    EqVal2 H (substExpr sigma M) (substExpr sigma' M) (substExpr sigma A) u a
-
-*)
-
-
+(* ValTy2-headred-expand *)
+Lemma ValTy_HeadRed_expand {n} (Γ : Ctx n) (M M' : Tm n) u (h : wt u tuniv) :
+  HeadRed M' M -> ValTy Γ M h -> ValTy Γ M' h.
+Proof. 
+  move=> R. induction R.
+  - done.
+  - move=> h1. specialize (IHR h1). 
+    eapply ValTy_HeadRed1_expand in H; eauto.
+Qed.
 
   
+
+Lemma ValTy_HeadRed1_contract {n} (Γ : Ctx n) (M M' : Tm n) u (h : wt u tuniv) :
+  HeadRed1 M M' -> ValTy Γ M h -> ValTy Γ M' h.
+Proof. 
+  move=> R. 
+  dependent destruction h.
+  all: cbn; try done.
+  move=> [A0 [B0 [R0 [TA0 [TB0 [Vpi [VA [PEV PEE]]]]]]]].
+  exists A0. exists B0.
+  repeat split; eauto.
+  eapply HeadRed_contract; eauto.
+Qed.
+
+
+
+(* ValTy2-headred-contract *)
+Lemma ValTy_headred_contract {n} (Γ : Ctx n) (M M' : Tm n) u (h : wt u tuniv) :
+  HeadRed M M' -> ValTy Γ M h -> ValTy Γ M' h.
+Proof. 
+  move=> R. induction R.
+  - done.
+  - admit.
+Admitted.
+
+
+(* ============================================================
+   upValTy / downValTy — stated before the mutual block.
+
+   Each is parameterized by the mutual-block lemma its proof
+   relies on, so it can be applied inside the mutual block by
+   passing the appropriate fixpoint reference at the call site.
+   ============================================================ *)
+
+(* downValTy: shrink the term-side element u (same type tuniv).
+   Derivable from [restrictVal] of the mutual block. *)
+Lemma downValTy_pre
+  (restrictVal :
+    forall n (Γ : Ctx n) (M T : Tm n) u u' a
+           (h0 : wt u' a) (h1 : wt u a),
+           le u' u -> Val Γ M T h1 -> Val Γ M T h0)
+  {n} (Γ : Ctx n) (M : Tm n) u0 u1
+  (h0 : wt u0 tuniv) (h1 : wt u1 tuniv) :
+  le u0 u1 -> ValTy Γ M h1 -> ValTy Γ M h0.
+Proof.
+  move=> LE VT1.
+  apply Val_ValTy. apply ValTy_Val in VT1.
+  eapply restrictVal; eauto.
+Qed.
+
+
+(* ============================================================
+   down/up
+   ============================================================ *)
+
+
+
+Lemma upValPi : forall 
+        (upVal : forall {n} (Γ : Ctx n) (M T : Tm n) u a0 a1
+                   (h0 : wt u a0) (h1 : wt u a1)  
+                   (hUa0 : wt a0 tuniv) (hUa1 : wt a1 tuniv), 
+            le a0 a1 -> Val Γ M T h0 -> Val Γ T Core.tuniv hUa1 -> Val Γ M T h1)
+        (downVal : forall {n} (Γ : Ctx n) (M T : Tm n) u a0 a1
+                     (h0 : wt u a0) (h1: wt u a1),
+            le a0 a1 -> Val Γ M T h1 -> Val Γ M T h0)
+        f a g a0 g0 
+        (LEa : le a a0) 
+        (LEg : le_fun g g0)           
+        (h  : wt (abs f) (tpi a g))
+        (h0 : wt (abs f) (tpi a0 g0))
+        (hUa1 : wt (tpi a0 g0) tuniv)
+        {n} (Γ : Ctx n) (M T : Tm n),
+        ValPi Γ M T h -> 
+        ValTy Γ T hUa1 ->
+        ValPi Γ M T h0.
+Proof.
+      move=> upVal downVal f a g a0 g0 LEa LEg h h0 hUa1 n Γ M T VP VTya1 .
+      dependent destruction hUa1.
+      destruct VTya1 as (Av & Bv & HRv & TAv & TBv & Vpi & VDv & PEV & PEE).        
+
+      unfold Rec.ValPi in VP.
+      destruct VP as (A0 & B0 & R1 & PAV).
+      (* types are the same *)
+      destruct (HeadRed_tpi_det HRv R1) as [-> ->].
+
+      unfold Rec.ValPi.
+      exists A0, B0.
+      repeat split; try eassumption.
+      move=> u v t0 Vu APP NB APPg0 N TN VN.
+      cbn. cbn in VN.
+
+      have WTpi : wt (tpi a g) tuniv.  eapply wt_ty_tuniv; eauto.
+      have Vg: valid_fun g. eapply valid_tpi2. eauto with valid.
+      have Vg0: valid_fun g0. eapply valid_tpi2. eauto with valid.
+      destruct (valid_app_exists Vg Vu) as [t [APPg Vt]].
+      have LEt: le t t0. { eapply (@le_fun_mono g g0 u); eauto. } 
+
+      have WTt: wt t tuniv. 
+      { destruct (is_bot t) eqn:EQ. destruct t; try done.
+        eapply wt_bot. eapply wt_tuniv.
+        inversion WTpi. eapply (H3 _ _ Vu); eauto. } 
+      have WTv: wt v t.
+      { inversion h. eapply (H3 u v t); eauto. } 
+      have NBt: ~(is_bot t).
+      { move=>IB. destruct t; try done. inversion WTv. subst. done. } 
+      have NBt0: ~(is_bot t0).
+      { move=>IB. destruct t0; destruct t; try done. }  
+      have WTu: wt u a0. { eauto. } 
+
+      unfold PiAppVal in PAV.
+      specialize (PAV u v t Vu APP NB APPg N TN).
+      specialize (PEV u t0 Vu APPg0 NBt0 WTu N TN).
+      cbn in PAV.
+      eapply upVal. 
+        ++ eapply WTt. 
+        ++ eapply LEt.
+        ++ eapply PAV.
+           eapply downVal. eapply LEa. eapply VN.
+        ++ eapply ValTy_Val. 
+           eapply PEV.
+           cbn.
+           erewrite (wt_unique (w u t0 Vu APPg0 NBt0)).
+           eapply VN.
+Defined.
+
+Lemma downValPi : forall 
+        (upVal : forall {n} (Γ : Ctx n) (M T : Tm n) u a0 a1
+                   (h0 : wt u a0) (h1 : wt u a1)  
+                   (hUa0 : wt a0 tuniv) (hUa1 : wt a1 tuniv), 
+            le a0 a1 -> Val Γ M T h0 -> Val Γ T Core.tuniv hUa1 -> Val Γ M T h1)
+        (downVal : forall {n} (Γ : Ctx n) (M T : Tm n) u a0 a1
+                     (h0 : wt u a0) (h1: wt u a1),
+            le a0 a1 -> Val Γ M T h1 -> Val Γ M T h0)
+        f a g a0 g0 
+        (LEa : le a a0) 
+        (LEg : le_fun g g0)           
+        (h  : wt (abs f) (tpi a g))
+        (h0 : wt (abs f) (tpi a0 g0))
+        (hUa : wt (tpi a g) tuniv)
+        {n} (Γ : Ctx n) (M T : Tm n),
+        ValPi Γ M T h0 -> 
+        ValTy Γ T hUa ->
+        ValPi Γ M T h.
+Proof.
+  move=> upVal downVal f a g a0 g0 LEa LEg h h0 hUa n Γ M T VP VT.
+  unfold Rec.ValPi in VP.
+  destruct VP as (A0 & B0 & R1 & PAV).
+  unfold ValPi.
+  exists A0, B0.
+  repeat split; try eassumption.
+
+  (* downPiAppVal *)
+  move=> u v t Vu APP NB APPg N TN VN.
+  cbn. cbn in VN.
+
+  have WTpi : wt (tpi a g) tuniv.  eapply wt_ty_tuniv; eauto.
+  have Vg: valid_fun g. eapply valid_tpi2. eauto with valid.
+  have Vg0: valid_fun g0. eapply valid_tpi2. eauto with valid.
+  destruct (valid_app_exists Vg0 Vu) as [t0 [APPg0 Vt0]].
+  have LEt: le t t0. { eapply (@le_fun_mono g g0 u); eauto. } 
+
+  have WTt: wt t tuniv. 
+  { destruct (is_bot t) eqn:EQ. destruct t; try done.
+    eapply wt_bot. eapply wt_tuniv.
+    inversion WTpi. eapply (H3 _ _ Vu); eauto. } 
+  have WTv: wt v t.
+  { inversion h. eapply (H3 u v t); eauto. } 
+  have NBt: ~(is_bot t).
+  { move=>IB. destruct t; try done. inversion WTv. subst. done. } 
+  have NBt0: ~(is_bot t0).
+  { move=>IB. destruct t0; destruct t; try done. }  
+  have WTa: wt a tuniv. inversion WTpi. done.
+  unfold PiAppVal in PAV.
+  specialize (PAV u v t0 Vu APP NB APPg0 N TN).
+
+  cbn in PAV.
+  eapply downVal. 
+  ++ eapply LEt.
+  ++ eapply PAV.
+     eapply upVal. eapply WTa. eapply LEa. eapply VN.
+Admitted.
+
+
+(* Annoyingly, struct on first derivation is not enough. Need
+   to do struct on *both* wt derivations simultaneously to
+   show the termination of this proof.
+
+   For now, admitting the termination check.
+*)
+
+(* upVal/upEqVal mirror the Agda upVal2/upEqVal2 signatures: they take
+   the ValTy of the syntactic type T at the bigger universe-element a1
+   as an extra argument (a "Val Γ T Core.tuniv hUa1", which by
+   definitional unfolding is ValTy Γ T hUa1).                          *)
+Fixpoint upVal {n} (Γ : Ctx n) (M T : Tm n) u a0 a1
+  (h0 : wt u a0) (h1 : wt u a1)  
+  (hUa0 : wt a0 tuniv) (hUa1 : wt a1 tuniv) {struct h1}:
+  le a0 a1 -> Val Γ M T h0 -> Val Γ T Core.tuniv hUa1 -> Val Γ M T h1
+with upEqVal {n} (Γ : Ctx n) (M N T : Tm n) u a0 a1
+  (h0 : wt u a0) (h1 : wt u a1)  
+  (hUa0 : wt a0 tuniv) (hUa1 : wt a1 tuniv) {struct h1}:
+  le a0 a1 -> EqVal Γ M N T h0 -> Val Γ T Core.tuniv hUa1 -> EqVal Γ M N T h1
+with downVal {n} (Γ : Ctx n) (M T : Tm n) u a0 a1
+  (h0 : wt u a0) (h1: wt u a1) {struct h1} :
+  le a0 a1 -> Val Γ M T h1 -> Val Γ M T h0
+with downEqVal {n} (Γ : Ctx n) (M N T : Tm n) u a0 a1
+  (h0 : wt u a0) (h1: wt u a1) {struct h1} :
+  le a0 a1 -> EqVal Γ M N T h1 -> EqVal Γ M N T h0
+with restrictVal {n} (Γ : Ctx n) (M T : Tm n) u u' a
+  (h0 : wt u' a) (h1 : wt u a) {struct h1} :
+  le u' u -> Val Γ M T h1 -> Val Γ M T h0
+with restrictEqVal {n} (Γ : Ctx n) (M N T : Tm n) u u' a
+  (h0 : wt u' a) (h1 : wt u a) {struct h1} :
+  le u' u -> EqVal Γ M N T h1 -> EqVal Γ M N T h0.
+Proof.  
+  - (* upVal *)
+    dependent destruction h1;
+    dependent destruction h0.
+    all: try solve [cbn; eauto].
+    + (* bot *)
+      destruct a; destruct a0; cbn; auto.
+    + (* tnat *)
+      move=> _ h3 _. cbn in h3. move: h3 => [M1 [RM1 VM1]].
+      exists M1. split. auto. 
+      cbn.
+      rewrite (wt_unique h0 h1) in VM1.
+      done.
+
+    + (* tuniv <= tuniv *)
+      move=> LE VT _.
+      cbn [Val] in VT |- *.
+      erewrite (wt_unique (wt_tpi h1 w1 w2 i0)).
+      eapply VT.
+      (* nothing to do here as only tuniv <= tuniv *)
+
+    + (* tpi a g <= tpi a0 g0 *)
+      dependent destruction h0.
+      dependent destruction h1.
+      rewrite le_tpi.
+      move=> LE. apply andb_prop in LE. destruct LE as [LEa LEg].
+      move=> VAL VTa1.
+      split.
+      * apply Val_ValTy in VTa1. 
+        erewrite (wt_unique hUa1) in VTa1.
+        eapply VTa1.
+      * (* need to use VTa1 *)
+        move: (Val_ValTy VTa1) => VTya1.
+        (* also need VP *)
+        cbn [Val] in VAL |- *. 
+        destruct VAL as [VT VP].
+        eapply (upValPi upVal downVal LEa LEg); eauto.
+
+  - (* upEqVal *)
+    dependent destruction h1;
+    dependent destruction h0.
+    all: try solve [cbn; eauto].
+    + (* bot *)
+      destruct a; destruct a0; cbn; auto.
+    + (* tnat *)
+      move=> _ [M1 [RM1 [N1 [RN1 EVM]]]] _.
+      exists M1. split. auto.
+      exists N1. split. auto.
+      rewrite (wt_unique h0 h1) in EVM.
+      done.
+    + (* tuniv <= tuniv *)
+      move=> LE EqV VT.
+      erewrite (wt_unique (wt_tpi h1 w1 w2 i0)).
+      eapply EqV.
+
+    + (* tpi a g <= tpi a0 g0 *)
+      dependent destruction h0.
+      dependent destruction h1.
+      rewrite le_tpi.
+      move=> LE. apply andb_prop in LE. destruct LE as [LEa LEg].
+      move=> EqVAL VTa1.
+      cbn [EqVal] in EqVAL |- *. 
+      destruct EqVAL as (VT & VPM & VPN & EVP).
+
+      apply Val_ValTy in VTa1. 
+      erewrite (wt_unique hUa1) in VTa1.
+      repeat split.
+      * eapply VTa1.
+      * eapply (upValPi upVal downVal LEa LEg); eauto. 
+      * eapply (upValPi upVal downVal LEa LEg); eauto. 
+      * (* need upEqValPi lemma *)
+        admit. 
+
+  - (* downVal *)
+    dependent destruction h1;
+    dependent destruction h0.
+    all: try solve [cbn; eauto].
+    + (* bot *)
+      destruct a; destruct a0; cbn; auto; done.
+    + (* tnat *)
+      move=> _ [M1 [RM1 VM1]].
+      exists M1. split. auto.
+      rewrite (wt_unique h1 h0) in VM1.
+      done.
+    + (* tuniv <= tuniv *)
+      move=> _ VT.
+      erewrite (wt_unique (wt_tpi h1 w1 w2 i0)) in VT.
+      eapply VT.
+    + (* tpi *)
+      dependent destruction h0.
+      dependent destruction h1.
+      rewrite le_tpi.
+      move=> LE. apply andb_prop in LE. destruct LE as [LEa LEg].
+      move=> VAL.
+      cbn [Val] in VAL |- *. 
+      destruct VAL as (VT & VP).
+      split.
+      * eapply Val_ValTy.
+        eapply ValTy_Val in VT.
+        eapply restrictVal; eauto.
+        rewrite le_tpi. rewrite LEa. rewrite LEg. done.
+      * eapply (downValPi upVal downVal LEa LEg); eauto. 
+        eapply Val_ValTy.
+        eapply ValTy_Val in VT.
+        eapply restrictVal; eauto.
+        rewrite le_tpi. rewrite LEa. rewrite LEg. done.
+
+  - (* downEqVal *)
+    dependent destruction h1;
+    dependent destruction h0.
+    all: try solve [cbn; eauto].
+    + destruct a; destruct a0; cbn; auto; done.
+    + move=> _ [M1 [RM1 [N1 [RN1 EVM]]]].
+      exists M1. split. auto.
+      exists N1. split. auto.
+      rewrite (wt_unique h1 h0) in EVM.
+      done.
+    + move=> _ EV.
+      erewrite (wt_unique (wt_tpi h0 w w0 i)).
+      eapply EV.
+    + (* tpi *)
+      dependent destruction h0.
+      dependent destruction h1.
+      rewrite le_tpi.
+      move=> LE. apply andb_prop in LE. destruct LE as [LEa LEg].
+      move=> VAL.
+      cbn [EqVal] in VAL |- *. 
+      destruct VAL as (VT & VPM & VPN & EVP).
+      repeat split.
+      * eapply Val_ValTy.
+        eapply ValTy_Val in VT.
+        eapply restrictVal; eauto.
+        rewrite le_tpi. rewrite LEa. rewrite LEg. done.
+      * eapply (downValPi upVal downVal LEa LEg); eauto. 
+        eapply Val_ValTy.
+        eapply ValTy_Val in VT.
+        eapply restrictVal; eauto.
+        rewrite le_tpi. rewrite LEa. rewrite LEg. done.
+      * eapply (downValPi upVal downVal LEa LEg); eauto. 
+        eapply Val_ValTy.
+        eapply ValTy_Val in VT.
+        eapply restrictVal; eauto.
+        rewrite le_tpi. rewrite LEa. rewrite LEg. done.
+      * (* downEqValPi *)
+        admit.
+  - (* restrictVal *)
+    dependent destruction h1.
+    (* bot <= bot *)
+    1: { move=> LE. apply le_bot_inv in LE. subst.
+         move=> h. erewrite (wt_unique h0). eapply h.
+    } 
+    all: dependent destruction h0.
+    all: try solve [cbn; done].
+    + (* succ <= succ *)
+      rewrite le_succ. move => LE VM.
+      destruct VM as [n1 [R1 T1]].
+      exists n1. split; auto.
+      cbn in T1 |- *. 
+      eapply restrictVal; eassumption.
+    + (* tpi a g <= tpi a0 g0 *)
+      rewrite le_tpi.
+      move=> /andP. move=> [LEa LEg].
+      move=> VM.
+      cbn [Val] in VM |- *.
+      destruct VM as (A & B & R1 & TA & TB & Vtpi & VA & PEV & PEE).
+      exists A. exists B. repeat split; eauto.
+      * (* PEV *)
+        move=> u v Vu APP NB WTu N TN VN.
+        have Vg : valid_fun g. eapply valid_tpi2. eauto. 
+        have Vg0 : valid_fun g0. eapply valid_tpi2. eauto. 
+        destruct (valid_app_exists Vg0 Vu) as [v0 [APP0 Vv0]].
+        move: (le_fun_mono Vg Vg0 LEg Vu APP APP0) => LEv.
+        have NB0: ~ (is_bot v0). { destruct v0; destruct v; try done. } 
+        have WTua0: wt u a0. eapply wt_le; eauto.
+        specialize (PEV _ _  Vu APP0 NB0 WTua0 N TN).
+        cbn in VN , PEV |- *.
+        eapply Val_ValTy.
+        eapply restrictVal; eauto.
+        eapply ValTy_Val.
+        eapply PEV.
+        eapply upVal. 3: eassumption. 2: eassumption. eapply wt_ty_tuniv; eauto.
+        eapply VA.
+      * (* PEE *) 
+        admit.
+    + (* abs f <= abs f0 *)
+      rewrite le_abs.
+      move=> LEf VM.
+      cbn in VM |- *.
+      move: VM => [ VTT VPM].
+      split.
+      * erewrite (wt_unique h0). eapply VTT.
+      * admit.
+  - (* restrictEqVal *)
+    admit.
+Admitted.
+
+
+(*
+
+
+      move=> LE EV.
+      cbn in EV |- *.
+      destruct EV as [VTm [VTn EVT]].
+      split; [|split].
+      * destruct VTm as (Am & Bm & RAm & TAm & TBm & Vpim & VVm & PEVm & PEEm).
+        rewrite (wt_pi_fun_unique w0 w) in PEVm, PEEm.
+        rewrite (wt_unique h1 h0) in VVm.
+        exists Am, Bm; repeat split; eassumption.
+      * destruct VTn as (An & Bn & RAn & TAn & TBn & Vpin & VVn & PEVn & PEEn).
+        rewrite (wt_pi_fun_unique w0 w) in PEVn, PEEn.
+        rewrite (wt_unique h1 h0) in VVn.
+        exists An, Bn; repeat split; eassumption.
+      * cbn in EVT |- *.
+        destruct EVT as (VTmE & VTnE & Ae & Be & RAe & Ae' & Be' & RAe' &
+                         CA & CB & VTpie & EVD & PEET).
+        split.
+        { destruct VTmE as (AmE & BmE & RAmE & TAmE & TBmE & VpimE & VVmE & PEVmE & PEEmE).
+          rewrite (wt_pi_fun_unique w0 w) in PEVmE, PEEmE.
+          rewrite (wt_unique h1 h0) in VVmE.
+          exists AmE, BmE; repeat split; eassumption. }
+        split.
+        { destruct VTnE as (AnE & BnE & RAnE & TAnE & TBnE & VpinE & VVnE & PEVnE & PEEnE).
+          rewrite (wt_pi_fun_unique w0 w) in PEVnE, PEEnE.
+          rewrite (wt_unique h1 h0) in VVnE.
+          exists AnE, BnE; repeat split; eassumption. }
+        exists Ae, Be; split; [exact RAe|].
+        exists Ae', Be'; split; [exact RAe'|].
+        rewrite (wt_pi_fun_unique w0 w) in PEET.
+        rewrite (wt_unique h1 h0) in EVD.
+        repeat split; eassumption.
+    + (* tpi *)
+      (* Mirror Agda Validity2.agda: downEqVal2 PiCode case.
+         EqVal at (abs f) (tpi a g) is
+            ValTy /\ ValPi M /\ ValPi N /\ EqValPi M N. *)
+      have Vtpi : valid (tpi a g). eauto with valid.
+      dependent destruction h0.
+      dependent destruction h1.
+      rewrite le_tpi.
+      move=> LE.
+      apply andb_prop in LE.
+      destruct LE as [LEa LEg].
+      move=> EVAL.
+      cbn in EVAL.
+      unfold Rec.ValPi, Rec.EqValPi in EVAL.
+      destruct EVAL as [VT [VPM [VPN EPI]]].
+      destruct VPM as [A0_M [B0_M [R_M PAV_M]]].
+      destruct VPN as [A0_N [B0_N [R_N PAV_N]]].
+      destruct EPI as [A0_E [B0_E [R_E PAEV]]].
+      cbn. split; [|split; [|split]].
+      * destruct VT as (Am & Bm & RAm & TAm & TBm & Vpim & VVm & PEVm & PEEm).
+        exists Am, Bm.
+        repeat split; try eassumption.
+        eapply restrictVal; eauto.
+        eapply downPiEdgeVal; eauto.
+        eapply downPiEdgeEq; eauto.
+      * unfold Rec.ValPi. exists A0_M, B0_M. split. exact R_M.
+        eapply downPiAppVal; eauto.
+      * unfold Rec.ValPi. exists A0_N, B0_N. split. exact R_N.
+        eapply downPiAppVal; eauto.
+      * unfold Rec.EqValPi. exists A0_E, B0_E. split. exact R_E.
+        eapply downPiAppEqVal; eauto.
+  - (* upPiAppVal: takes extra PiEdgeVal 
+       at the bigger pi (mirror of Agda's piEV1). *)
+    intros LE LEg piEV1 PA.
+    dependent destruction h0.
+    + (* wt_abs_nil *) dependent destruction h1. cbn. trivial.
+    + (* wt_abs_cons *)
+      dependent destruction h1.
+      cbn in PA. destruct PA as [PA_rec PA_forall].
+      cbn. split.
+      * (* Tail recursion: pass the OUTER hPi0/hPi1 (unchanged, since g/b are
+           preserved) and the TAIL h0/h1 (subderivations from dep destr). *)
+        exact (@upPiAppVal _ _ _ _ _ _ _ _ _ _ hPi0 hPi1 h0 h1 LE LEg piEV1 PA_rec).
+      * 
+        move=> P TP VP1.
+        move: (@downVal _ Γ P A0 ui a a0 w w1 LE VP1) => VP.
+        specialize (PA_forall P TP VP).
+        have Vg: valid_fun g. eapply valid_tpi2. eauto with valid.
+        have Vg0: valid_fun g0. eapply valid_tpi2. eauto with valid.
+        have LEt: le t t0.
+        { eapply (@le_fun_mono g g0); eauto. 
+          eauto with valid. } 
+        have WTt0: wt t0 tuniv. eapply wt_ty_tuniv; eauto.
+        have LEMMA : forall n (Γ : Ctx n) P A0 B0 g0 a0 ui t0
+             (hPi1 : wt_pi_fun g0 a0)
+             (piEV1 : PiEdgeVal Γ A0 B0 hPi1)
+             (e0 : app g0 ui = Some t0)
+             (w1 : wt ui a0)
+             (WTt0 : wt t0 tuniv),
+             (typing Γ P A0) -> 
+             (Val Γ P A0 w1) ->
+             Val Γ B0[P..] Core.tuniv WTt0.
+        { clear. 
+          move=> n Γ P A0 B0 g0.
+          all: move=> a0 ui t0 hPi1 PEV APP w1 w2 T1 V1.
+          - admit.
+          - move=> APP w1 WTt0 TO VP.
+            destruct a as [u v].
+            inversion hPi1. subst. 
+            rewrite app_cons_eq in APP.
+        } 
+        have ValT: Val Γ B0[P..] Core.tuniv WTt0.
+        { eapply LEMMA; eauto.  } 
+        eapply upVal. 2: exact LEt. 
+        eapply wt_ty_tuniv; eauto.
+        eauto.
+        eauto.
+
+  - (* downPiAppVal *)
+    intros LE LEg PA.
+    dependent destruction h1.
+    + dependent destruction h0. cbn. trivial.
+    + dependent destruction h0.
+      cbn in PA. destruct PA as [PA_rec PA_forall].
+      cbn. split.
+      * (* Tail recursion on the wt_abs_fun tails h0, h1 (subderivations). *)
+        exact (@downPiAppVal _ _ _ _ _ _ _ _ _ _ h0 h1 LE LEg PA_rec).
+      * admit.
+  - (* upPiAppEq *)
+    intros LE LEg PEV PA.
+    dependent destruction h0.
+    + dependent destruction h1. cbn. trivial.
+    + dependent destruction h1.
+      cbn in PA. destruct PA as [PA_rec PA_forall].
+      cbn. split.
+      * exact (@upPiAppEq _ _ _ _ _ _ _ _ _ _ hPi0 hPi1 h0 h1 LE LEg PEV PA_rec).
+      * admit.
+  - (* downPiAppEq *)
+    intros LE LEg PA.
+    dependent destruction h1.
+    + dependent destruction h0. cbn. trivial.
+    + dependent destruction h0.
+      cbn in PA. destruct PA as [PA_rec PA_forall].
+      cbn. split.
+      * exact (@downPiAppEq _ _ _ _ _ _ _ _ _ _ h0 h1 LE LEg PA_rec).
+      * admit.
+  - (* upPiAppEqVal *)
+    intros LE LEg PEV PA.
+    dependent destruction h0.
+    + dependent destruction h1. cbn. trivial.
+    + dependent destruction h1.
+      cbn in PA. destruct PA as [PA_rec PA_forall].
+      cbn. split.
+      * exact (@upPiAppEqVal _ _ _ _ _ _ _ _ _ _ _ hPi0 hPi1 h0 h1 LE LEg PEV PA_rec).
+      * admit.
+  - (* downPiAppEqVal *)
+    intros LE LEg PA.
+    dependent destruction h1.
+    + dependent destruction h0. cbn. trivial.
+    + dependent destruction h0.
+      cbn in PA. destruct PA as [PA_rec PA_forall].
+      cbn. split.
+      * exact (@downPiAppEqVal _ _ _ _ _ _ _ _ _ _ _ h0 h1 LE LEg PA_rec).
+      * admit.
+  - (* downPiEdgeVal *)
+    intros LE LEf PE.
+    dependent destruction h0.
+    + (* wt_pi_nil: PiEdgeVal at nil is True *)
+      cbn. trivial.
+    + (* wt_pi_cons: needs to find a corresponding entry in h1 via le_fun;
+         the forall-part also needs cross-witness Val transport. *)
+      admit.
+  - (* downPiEdgeEq *)
+    intros LE LEf PE.
+    dependent destruction h0.
+    + cbn. trivial.
+    + admit.
+  - (* downPiEdgeEqTy *)
+    intros LE LEf PE.
+    dependent destruction h0.
+    + cbn. trivial.
+    + admit.
+  - (* restrictVal: shrink the term-side u (same a, smaller u' ≤ u). *)
+    admit.
+  - (* restrictEqVal *)
+    admit.
+Admitted.
+
+
+(* ---- down on ValTy / EqValTy ---- *)
+
+(* downValTy2 *)
+Lemma downValTy {n} (Γ : Ctx n) (M : Tm n) u0 u1 
+  (h0 : wt u0 tuniv) (h1 : wt u1 tuniv) :
+  le u0 u1 -> ValTy Γ M h1 -> ValTy Γ M h0.
+Proof.
+    move=> LE VT1.
+    eapply Val_ValTy.
+    apply ValTy_Val in VT1.
+    eapply restrictVal; eauto.
+Qed.
+
+(* downEqValTy2 *)
+Lemma downEqValTy {n} (Γ : Ctx n) (M N : Tm n) u0 u1 
+  (h0 : wt u0 tuniv) (h1 : wt u1 tuniv) :
+  le u0 u1 -> EqValTy Γ M N h1 -> EqValTy Γ M N h0.
+Proof.
+    move=> LE VT1.
+    eapply EqVal_EqValTy.
+    apply EqValTy_EqVal in VT1.
+    eapply restrictEqVal; eauto.
+Qed.
+*)
+
+
+(* ValTy2-Sup: if a1 and a2 are universe-members and lub a1 a2 = Some a,
+   ValTy at a1 and a2 lifts to ValTy at the lub. *)
+Fixpoint ValTy_Sup {n} (Γ : Ctx n) (T : Tm n) a1 a2 a 
+  (h1 : wt a1 tuniv) (h2 : wt a2 tuniv) (h : wt a tuniv) {struct h}:
+  lub a1 a2 = Some a ->
+  ValTy Γ T h1 -> ValTy Γ T h2 -> ValTy Γ T h.
+Proof.
+Abort.
+
+(* EqValTy2-Sup *)
+Lemma EqValTy_Sup {n} (Γ : Ctx n) (M N : Tm n) a1 a2 a 
+  (h1 : wt a1 tuniv) (h2 : wt a2 tuniv) (h : wt a tuniv) :
+  lub a1 a2 = Some a ->
+  EqValTy Γ M N h1 -> EqValTy Γ M N h2 -> EqValTy Γ M N h.
+Proof. 
+Abort.
+
+
+(* ----------------------------------------------------- *)
+
+Fixpoint Val_EqVal_fwd {n} (Γ : Ctx n) (M A : Tm n) u a
+  (h : wt u a) (B : Tm n)  (h' : wt a tuniv)
+  {struct h} :
+  Val Γ M A h -> EqValTy Γ A B h' -> Val Γ M B h
+with EqVal_EqVal_fwd {n} (Γ : Ctx n) (M N A : Tm n) u a
+  (h : wt u a) (B : Tm n)  (h' : wt a tuniv)
+  {struct h} :
+  EqVal Γ M N A h -> EqValTy Γ A B h' -> EqVal Γ M N B h
+with EqVal_sym {n} (Γ : Ctx n) (M1 M2 A : Tm n) u a (h : wt u a) { struct h } :
+  EqVal Γ M1 M2 A h -> EqVal Γ M2 M1 A h
+with EqVal_trans {n} (Γ : Ctx n) (M1 M2 M3 A : Tm n) u a (h : wt u a) {struct h} :
+  EqVal Γ M1 M2 A h -> EqVal Γ M2 M3 A h -> EqVal Γ M1 M3 A h.
+Proof.
+  - (* Val_EqVal_fwd *)
+    move=> VM EVTA.
+    dependent destruction h';
+      dependent destruction h.
+    all: try solve [cbn; try done].
+    cbn [EqValTy] in EVTA.
+    cbn in VM  |- *.
+    move: EVTA => [VTA [VTB [A0 [B0 [R0 [A1 [B1 [R1 [CA [CB [Vtpi [EVA PEET]]]]]]]]]]]].
+    split.
+    * erewrite (wt_unique h). eapply VTB.
+    * unfold ValPi.
+      exists A1, B1. split; auto.
+      unfold Rec.PiAppVal.
+      move=> u v t Vu APP NB APPg P TP VP.
+      specialize (PEET u t Vu APPg).
+      move: (w0 u v t Vu APP NB APPg) => WTv.
+      have NBt : ~ (is_bot t).
+      { destruct v; destruct t; inversion WTv; try done. } 
+      specialize (PEET NBt P). cbn in PEET |- *. cbn in VP. cbn in EVA.
+      admit.
+  - (* EqVal_EqVal_fwd *)
+    admit.
+  - (* EqVal_sym *)
+    admit.
+  - (* EqVal_trans *)
+    admit.
+Admitted.
+
+
+
+(* EqValTy2-sym *)
+Lemma EqValTy_sym {n} (Γ : Ctx n) (M N : Tm n) u (h : wt u tuniv) :
+  EqValTy Γ M N h -> EqValTy Γ N M h.
+Proof.
+  move=>h1. eapply EqVal_EqValTy. eapply EqVal_sym.
+  eapply EqValTy_EqVal. done.
+Qed.
+
+(* EqValTy2-trans *)
+Lemma EqValTy_trans {n} (Γ : Ctx n) (A B C : Tm n) u (h : wt u tuniv) :
+  EqValTy Γ A B h -> EqValTy Γ B C h -> EqValTy Γ A C h.
+Proof.
+  move=> h1 h2.
+  eapply EqVal_EqValTy. eapply EqVal_trans.
+  eapply EqValTy_EqVal. eauto.
+  eapply EqValTy_EqVal. eauto.
+Qed.
+
+(* ============================================================
+   Translations of theorem statements from Validity2.agda
+   ------------------------------------------------------------
+
+   Translation conventions (Agda → Rocq):
+     FinMem u a              ≈  wt u a
+     FinMem b UCode          ≈  wt b tuniv         (some i)
+     Coherent u              ≈  valid u                (implicit in wt)
+     CoherentFun g           ≈  valid_fun g            (implicit in wt (abs g) ..)
+     CoherentFunTail f       ≈  valid_fun f            (implicit in wt (tpi _ f) ..)
+     FinMemFun g b f         ≈  wt (abs g) (tpi b f)
+     FinMemAllU f b          ≈  wt (tpi b f) tuniv (codomains in U_i)
+     LeCode u v              ≈  le u v
+     LeFunCode f g           ≈  le_fun f g
+     Comp u v                ≈  compatible u v
+     Sup u v = w             ≈  lub u v = Some w
+     Selection f u v         ≈  In (u, v) f
+     EvalFun f u = v         ≈  app f u = Some v
+     subst1 B N              ≈  B[N..]
+     HasType / ConvTm        ≈  typing / conv
+     HeadRed                 ≈  HeadRed (multi reduction)
+
+   Closed terms (Tm 0) are used throughout.
+
+   ------------------------------------------------------------
+   Dependency stratification of the mutual block.
+
+   The Agda mutual block of Validity2.agda decomposes into the
+   following strongly-connected components, in topological order
+   (a level may only call itself or earlier levels):
+
+     Level 1 (no recursive calls in the mutual block):
+       - EqVal_Val1                   (Val2-from-EqVal2-first)
+       - EqVal_Val2                   (Val2-from-EqVal2-second)
+       - ValTy_headred_expand         (ValTy2-headred-expand)
+       - ValTy_headred_contract       (ValTy2-headred-contract)
+
+     Level 2 (calls into Level 1 only):
+       - EqValTy_headred_expand       (uses ValTy_headred_expand)
+       - EqValTy_headred_contract     (uses ValTy_headred_contract)
+
+     Level 3 (4-way SCC, plus dependencies on Levels 1-2):
+       Val_beta_expand  ↔  ValPi_headred_expand
+                        ↔  EqVal_headred_expand
+                        ↔  EqValPi_headred_expand
+
+     Level 4 (4-way SCC, plus dependencies on Levels 1-2):
+       Val_headred_contract  ↔  ValPi_headred_contract
+                             ↔  EqVal_headred_contract
+                             ↔  EqValPi_headred_contract
+
+     Level 5 (2-way SCC, independent of Levels 3-4):
+       Val_EqVal  ↔  ValTy_EqValTy
+
+     Level 6 (BIG SCC, ~30 lemmas, depends only on Levels 1, 5):
+       { EqValTy_sym, EqValTy_trans, EqVal_sym, EqVal_trans,
+         Val_EqVal_fwd, EqVal_EqVal_fwd, ValTy_Sup, EqValTy_Sup,
+         downVal, downEqVal, downValTy, downEqValTy,
+         upVal, upEqVal, restrictVal, restrictEqVal,
+         downPiAppVal, downPiAppEq, downPiAppEqVal,
+         upPiAppVal, upPiAppEq, upPiAppEqVal,
+         transportPiEdgeVal_sel, transportPiEdgeEq_sel,
+         transportPiEdgeEqTy_sel,
+         restrictPiAppVal_sel, restrictPiAppEq_sel,
+         restrictPiAppEqVal_sel,
+         restrictVal_PiCode, restrictEqVal_PiCode }
+
+     Cycles in Level 6 (sample):
+       downVal → downValTy → transportPiEdgeVal_sel → upVal
+              → upPiAppVal → downVal
+       restrictVal → restrictVal_PiCode → restrictPiAppVal_sel
+                   → restrictVal
+       Val_EqVal_fwd → restrictVal → upPiAppVal → ... → Val_EqVal_fwd
+   ============================================================ *)
+
+
+
+(* ============================================================
+   Level 2 — depends on Level 1
+   ============================================================ *)
+
+(* EqValTy2-headred-expand *)
+Lemma EqValTy_headred_expand {n} (Γ : Ctx n) (M1 M2 M1' M2' : Tm n) u 
+  (h : wt u tuniv) :
+  HeadRed M1' M1 -> HeadRed M2' M2 ->
+  EqValTy Γ M1 M2 h -> EqValTy Γ M1' M2' h.
+Proof. Admitted.
+
+(* EqValTy2-headred-contract *)
+Lemma EqValTy_headred_contract {n} (Γ : Ctx n) (M1 M2 M1' M2' : Tm n) u 
+  (h : wt u tuniv) :
+  HeadRed M1 M1' -> HeadRed M2 M2' ->
+  EqValTy Γ M1 M2 h -> EqValTy Γ M1' M2' h.
+Proof. Admitted.
+
+
+(* ============================================================
+   Level 3 — 4-way SCC for HeadRed expand on Val/EqVal/ValPi/EqValPi
+   ============================================================ *)
+
+(* Val2-beta-expand *)
+Lemma Val_beta_expand {n} (Γ : Ctx n) (M M' T : Tm n) u a (h : wt u a) :
+  HeadRed M' M -> Val Γ M T h -> Val Γ M' T h.
+Proof. Admitted.
+
+(* EqVal2-headred-expand *)
+Lemma EqVal_headred_expand {n} (Γ : Ctx n) (M M' N N' T : Tm n) u a (h : wt u a) :
+  HeadRed M' M -> HeadRed N' N ->
+  EqVal Γ M N T h -> EqVal Γ M' N' T h.
+Proof. Admitted.
+
+(* ValPi2-headred-expand *)
+Lemma ValPi_headred_expand {n} (Γ : Ctx n) (M M' T : Tm n) b f g
+  (h : wt (abs g) (tpi b f)) :
+  HeadRed M' M -> ValPi Γ M T h -> ValPi Γ M' T h.
+Proof. Admitted.
+
+(* EqValPi2-headred-expand *)
+Lemma EqValPi_headred_expand {n} (Γ : Ctx n) (M1 M2 M1' M2' T : Tm n) b f g
+  (h : wt (abs g) (tpi b f)) :
+  HeadRed M1' M1 -> HeadRed M2' M2 ->
+  EqValPi Γ M1 M2 T h -> EqValPi Γ M1' M2' T h.
+Proof. Admitted.
+
+
+(* ============================================================
+   Level 4 — 4-way SCC for HeadRed contract
+   ============================================================ *)
+
+(* Val2-headred-contract *)
+Lemma Val_headred_contract {n} (Γ : Ctx n) (M M' T : Tm n) u a (h : wt u a) :
+  HeadRed M M' -> Val Γ M T h -> Val Γ M' T h.
+Proof. Admitted.
+
+(* EqVal2-headred-contract *)
+Lemma EqVal_headred_contract {n} (Γ : Ctx n) (M M' N N' T : Tm n) u a (h : wt u a) :
+  HeadRed M M' -> HeadRed N N' ->
+  EqVal Γ M N T h -> EqVal Γ M' N' T h.
+Proof. Admitted.
+
+(* ValPi2-headred-contract *)
+Lemma ValPi_headred_contract {n} (Γ : Ctx n) (M M' T : Tm n) b f g
+  (h : wt (abs g) (tpi b f)) :
+  HeadRed M M' -> ValPi Γ M T h -> ValPi Γ M' T h.
+Proof. Admitted.
+
+(* EqValPi2-headred-contract *)
+Lemma EqValPi_headred_contract {n} (Γ : Ctx n) (M1 M2 M1' M2' T : Tm n) b f g
+  (h : wt (abs g) (tpi b f)) :
+  HeadRed M1 M1' -> HeadRed M2 M2' ->
+  EqValPi Γ M1 M2 T h -> EqValPi Γ M1' M2' T h.
+Proof. Admitted.
+
+
