theories/examples/finelt/types.v
@@ -5,6 +5,7 @@ Set Implicit Arguments.
 Unset Strict Implicit.
 Unset Printing Implicit Defensive.
 
+From Stdlib Require Import ProofIrrelevance.
 
 From Stdlib Require Import Classes.RelationClasses Classes.Morphisms Lia Arith.
 
@@ -16,57 +17,32 @@ Require Import findom.
 
 Import findom.Raw.
 
+(* Note about minimality / function representation
+ 
+   For some functions: we might want this property
+ 
+    (ui,vi) in f, (uj,vj) in f,   ui <= uj implies vi <= vj 
+
+   This gives us for any (ui,vi) in f,
+    app f ui = Some vi    
+    (* exactly, don't need to look at other tuples *)
+
+    
+   example: consider F:
+     (succ (succ bot),  { (1,1) }  )
+     (succ bot, { (0,0) } )
+
+
+   minimal but violates the property because 
+      F (suc (succ bot)) = { (0,0), (1,1) }
+
+   this property + minimal means unique representation for sets of pairs
+   
+*)
 
 
 (* -------------------------------------------------------------- *)
 
-(*
-Fixpoint wt_tpi' (wt: elt -> elt -> Prop) b g i : Prop :=
-    match g with 
-    | ((u,v) :: g') => wt u b /\ wt v (tuniv i) /\ wt_tpi' wt b g' i
-    | nil => True
-    end.
-Fixpoint wt_abs' (wt:elt -> elt -> Prop) f a g : Prop := 
-    match f with 
-    | (u,v) :: f' => wt u a 
-                     /\ exists w, app g u = Some w /\ wt v w
-                     /\ wt_abs' wt f' a g
-    | nil => True
-    end.
-
-Fixpoint wt (u:elt) (a : elt) { struct u } : Prop := 
-  match u with 
-  | bot => valid a
-  | tuniv i => match a with 
-               | tuniv j => (i < j)%nat
-               | _ => False
-              end
-  | tpi b g => 
-      match a with 
-      | tuniv i => 
-          wt_tpi' wt b g i /\ wt b (tuniv i)
-          /\ valid (tpi b g) 
-      | _ => False 
-      end    
-  | abs f => 
-      match a with 
-      | tpi b g =>  
-          wt_abs' wt f b g /\
-          valid (abs f) /\ valid (tpi b g) 
-      | _ => False
-      end
-  | _ => False
-end.
-
-Notation wt_tpi := (wt_tpi' wt).
-Notation wt_abs := (wt_abs' wt).
-*)
-
-Fixpoint ForallT (A : Type) (P : A -> Type) (l : list A) : Type :=
-  match l with
-  | nil => True
-  | x :: l => P x * ForallT P l
-  end.
 
 (** well typed elements (finMem)
     In this branch tuniv has no universe-level argument (type-in-type). *)
@@ -106,7 +82,7 @@ Inductive wt : elt -> elt -> Type :=
     wt (tpi a g) tuniv ->
     wt (abs f) (tpi a g).
 
-From Stdlib Require Import ProofIrrelevance.
+
 
 (* Uniqueness of [wt] (and its mutual companions) derivations.
    Constructors that hold positive content recurse on the sub-derivations;
@@ -130,53 +106,8 @@ Fixpoint wt_unique u a (h1 h2 : wt u a) {struct h1} : h1 = h2.
 Qed.
 
 
-(* app f ui = lub { vj | uj <= ui  and (uj,vj) in f } *)
+(** * Validity *)
 
-(* For some functions: we might want this property
- 
-    (ui,vi) in f, (uj,vj) in f,   ui <= uj implies vi <= vj 
-
-   This gives us for any (ui,vi) in f,
-    app f ui = Some vi    
-    (* exactly, don't need to look at other tuples *)
-
-    
-   example: consider F:
-     (succ (succ bot),  { (1,1) }  )
-     (succ bot, { (0,0) } )
-
-
-   minimal but violates the property because 
-      F (suc (succ bot)) = { (0,0), (1,1) }
-
-   this property + minimal means unique representation for sets of pairs
-   
-*)
-
-(* If we restrict to these elements, then we can think about this 
-   stronger typing rule for functions *)
-(*
-Lemma wt_abs_ext a f g :
-    (forall u, exists v, wt v a /\ app f u = app f v) ->
-    (forall u w v, app g u = Some w -> app f u = Some v -> wt v w) ->
-    (* make sure both tm and type are valid *)
-    (valid (abs f)) ->
-    (valid (tpi a g)) <-> 
-    wt (abs f) (tpi a g)
-  .
-Abort.
-*)
-
-Lemma valid_tpi1 a g : valid (tpi a g) -> valid a.
-move=> /andP [h1 h2]. exact h1.
-Qed.
-Lemma valid_tpi2 a g : valid (tpi a g) -> valid_fun g.
-move=> /andP [h1 h2]. exact h2.
-Qed.
-Lemma valid_abs f : valid (abs f) -> valid_fun f.
-move=> /andP [h1 _]. exact h1.
-Qed.
-Hint Resolve valid_tpi1 valid_tpi2 valid_abs : valid.
 
 Fixpoint wt_valid_tm u a : wt u a -> valid u.
 - induction 1; eauto.  
@@ -192,268 +123,66 @@ Hint Resolve wt_valid_tm wt_valid_ty : valid.
 Lemma wt_bot_inv u : wt u bot -> u = bot.
 Proof. move=> h. inversion h. done. Qed.
 
+(** Generation / regularity *)
+
 (* FinMem-a-in-U (type-in-type: every typed term's type lives in tuniv). *)
 Lemma wt_ty_tuniv u a : wt u a -> wt a tuniv.
 Proof.
   induction 1; eauto using wt_tuniv, wt_tnat, wt_tpi.
 Qed.
 
+(** ** Inversion lemmas *)
 
-Lemma In_rk_fun1 u v f:
-  In (u, v) f -> rk u <= rk_fun f.
+
+Lemma wt_succ_inv u:
+  wt (succ u) tnat -> wt u tnat.
+move=>h. inversion h. done. Defined.
+
+Lemma wt_abs_ty g b f : 
+  wt (abs g) (tpi b f) -> wt (tpi b f) tuniv.
+Proof. 
+  move=> h. inversion h. eauto.
+Defined.
+
+
+Lemma wt_abs_inv1 g a f : 
+  wt (abs f) (tpi a g) ->     
+  (forall u v, valid u -> app f u = Some v -> ~ is_bot v -> wt u a).
+Proof. 
+  move=> h. inversion h. eauto.
+Defined.
+
+Lemma wt_abs_inv2 g a f : 
+  wt (abs f) (tpi a g) ->    
+  (forall u v t, valid u -> app f u = Some v -> ~ is_bot v -> app g u = Some t -> wt v t). 
+Proof. 
+  move=> h. inversion h. eauto.
+Defined.
+
+
+Lemma wt_tpi_dom a g :
+  wt (tpi a g) tuniv  -> wt a tuniv.
 Proof.
-  induction f as [|[ui vi]f]; eauto. cbn. done.
-  move=> [h1|h1].
-  inversion h1; subst. cbn. lia.
-  apply IHf in h1. cbn. lia.
-Qed.
+  move=> h. inversion h. eauto.
+Defined.
 
-Lemma In_rk_fun2 u v f:
-  In (u, v) f -> rk v <= rk_fun f.
+
+Lemma wt_tpi_inv1 a g :
+  wt (tpi a g) tuniv -> 
+  (forall u v, valid u -> app g u = Some v -> ~ is_bot v -> wt u a).
 Proof.
-  induction f as [|[ui vi]f]; eauto. cbn. done.
-  move=> [h1|h1].
-  inversion h1; subst. cbn. lia.
-  apply IHf in h1. cbn. lia.
-Qed.
+  move=> h. inversion h. eauto.
+Defined.
 
-Lemma rk_abs f : 
-  valid (abs f) -> 1 <= rk_fun f.
+Lemma wt_tpi_inv2 a g :
+  wt (tpi a g) tuniv -> 
+  (forall u v, valid u -> app g u = Some v -> ~ is_bot v -> wt v tuniv).
 Proof.
-  move=> /andP [Vf Nf]. fold valid (valid_fun f) in Vf.
-  destruct f as [|[u v]f]. done.
-  apply valid_fun_head in Vf.
-  apply val_nbot in Vf.
-  cbn.
-  destruct v; try done.
-  all: cbn.
-  all: lia.
-Qed.
+  move=> h. inversion h. eauto.
+Defined.
 
-(*
-Module WTL.
 
-Record WTLemmas k := MkLemmas { 
-    wt_le  : forall u a b, max (rk u) (max (rk a) (rk b)) <= k -> wt u a -> 
-       le a b -> forall i, wt a (tuniv i) -> wt b (tuniv i) -> wt u b ;
-    wt_lub : forall u a, max (rk u) (rk a) <= k -> wt u a -> 
-       forall v w, wt v a -> lub u v = Some w -> wt w a ;
-    wt_instantiate : 
-       forall b f i ui, wt (tpi b f) (tuniv i) ->                
-             wt ui b -> 
-             max (rk (tpi b f)) (rk ui) <= k ->
-             forall w, app f ui = Some w -> wt w (tuniv k) ;
-    wt_app : forall f b g u, max (rk_fun f) (max (rk (tpi b g)) (rk u)) <= k ->
-            wt (abs f) (tpi b g) -> wt u b -> 
-            forall t r, app g u = Some r -> app f u = Some t -> wt r t 
-}.
-
-(*
-finMemFun-upward : (g : FinFun) (a b : FinEl) (f h : FinFun) ->
-  LeCode a b -> Coherent a -> Coherent b ->
-  CoherentFunTail f -> CoherentFunTail h -> LeFunCode f h ->
-  FinMemFun g a f -> FinMem b UCode -> FinMemAllU h b -> FinMemFun g b h
-*)
-
-Definition wt_fun g a f := 
-   (forall ui vi, 
-        List.In (ui,vi) g -> wt ui a) /\
-    (forall ui vi w, 
-        List.In (ui,vi) g -> app f ui = Some w -> wt vi w).
-
-Lemma wt_le_fun : forall g a b f h i, 
-    le a b -> valid a -> valid b -> valid_fun f -> valid_fun h -> 
-    le_fun f h -> 
-    wt_fun g a f ->
-    wt (tpi b h) (tuniv i) -> 
-    wt_fun g b h.
-Proof.
-  induction g as [|[u v]g].
-  - intros. split; intros; done.
-  - move=> a b f h i LEa Va Vb Vf Vh LEf [WTg1 WTg2] WTP.
-    split.
-    + admit.
-    + move=> ui vi w [h1|h2] APP.
-      -- inversion h1.  subst. clear h1.
-         destruct (valid_app_exists Vf Vui) as [w [APPf Vw]].
-         move: (le_fun_mono Vf Vh LEf APP)
-         specialize (WTg2 _ _ _ ltac:(left; eauto)
-      -- 
-
-Lemma WTLs : forall k, WTLemmas k.
-Proof.
-  elim /strong_ind.
-  move=> m ih.
-  constructor.
-  - (* wt_le *)
-    move=> u a b RK WTu LE i0 WTa WTb.
-    dependent destruction WTu.
-    + eapply wt_bot; eauto. 
-    + apply le_tuniv_inv in LE. subst. 
-      eapply wt_tuniv; eauto.
-    + apply le_tuniv_inv in LE. subst.
-      eapply wt_tnat; eauto.
-    + apply le_tnat_inv in LE. subst.
-      eapply wt_zero; eauto.
-    + eapply le_tnat_inv in LE. subst.
-      eapply wt_succ; eauto.
-    + apply le_tuniv_inv in LE. subst.    
-      eapply wt_tpi; eauto.
-    + (* abs case: know wt (abs f) (tpi a g), 
-         WTP wt (abs f) (tpi a1 g1) where a <= a1 and g <= g1  *)
-      destruct (le_tpi_inv LE) as [a1 [g1 [-> [LEa LEg]]]].
-      cbn in RK. fold rk rk_fun in RK. 
-      
-
-      have WTpi: wt (tpi a g) (tuniv (max i0 i)).
-      { eapply wt_cumul; eauto. lia. }
-      have WTpi1: wt (tpi a1 g1) (tuniv (max i0 i)).
-      { eapply wt_cumul; eauto. lia. }
-      
-      have Vf: valid_fun f. eauto with valid.
-      have Vtpi1: valid (tpi a1 g1). eauto with valid.
-      have Vg1 : valid_fun g1. eapply valid_tpi2; eauto.  
-      have Vtpi : valid (tpi a g). eauto with valid.
-      have Vg : valid_fun g. eapply valid_tpi2; eauto.
-      
-      eapply wt_abs; eauto.
-      ++ (* dom elts are wt ui a1 *)
-        move=> ui vi Inf.
-        have RKui : rk ui <= rk_fun f. eapply In_rk_fun1; eauto.
-        have RKvi : rk vi <= rk_fun f. eapply In_rk_fun2; eauto.
-        have Vui: valid ui. eauto with valid.
-        move: (valid_app_exists Vg Vui) => [wi [Ai Vwi]].
-        eapply wt_le; eauto. lia.
-        inversion WTa. eauto.
-        inversion WTb. eauto.
-    ++ (* rng elts are wt *)
-      move=> ui vi w1 Inf APP1.
-      have RKui : rk ui <= rk_fun f. eapply In_rk_fun1; eauto.
-      have RKvi : rk vi <= rk_fun f. eapply In_rk_fun2; eauto.
-      have Vui: valid ui. eauto with valid.
-      move: (valid_app_exists Vg Vui) => [w [APP Vw]].
-      move: (rk_app APP) => RKw.
-      move: (rk_app APP1) => RKw1.
-      move: (rk_abs H1) => RKf.
-      have WTvi: wt vi w. 
-      { eapply H0; eauto. } 
-      have LFM: le w w1. 
-      { eapply (le_fun_mono Vg Vg1 LEg Vui APP APP1). } 
-      (* Given wt vi w and w <= w1 want to show wt vi w1 *)
-
-      (* BUT to apply IH (i.e. H2) we need to know that 
-         both w and w1 have a common universe level. *)
-      (* we know that w is good by assumption *)
-      have [j WTw] : exists j, wt w (tuniv j).
-      { eapply wt_ty_tuniv; eauto.  } 
-
-      (* but we need to somehow know that w1 is well typed. *)
-      have WTw1: wt w1 (tuniv i0).
-      { specialize (ih (max (rk_fun f) (max (max (rk a) (rk_fun g)) 
-                                          (max (rk a1) (rk_fun g1)))) ltac:(lia)).
-        move: (@wt_instantiate _ ih _ _ _ _ WTb) => LTI. 
-        cbn in LTI. fold rk_fun in LTI.
-        specialize (LTI ltac:(lia)).
-        
-        
-admit.  (* app g1 ui = w1i and  
-                         where wt (tpi a g1) (tuniv i0) *) }  
-
-      destruct (~~ is_nil g) eqn:Ng_g.
-      -- destruct (~~ is_nil g1) eqn:Ng_g1.
-         ++ 
-            Unshelve.
-            have Vw1i: valid w1i by eapply (valid_app Vg1 Vui A1i).
-            move: (wt_ty_tuniv WTvi) => [j WTwi].
-            move: (H2 _ _ _ Inf Ai) => Hwt.
-            have WTwi': (wt wi (tuniv (max (max i0 i) j))).
-            { eapply wt_cumul. eauto. lia. } clear WTwi.
-            eapply H2; eauto.
-            eapply wt_cumul. eauto. lia.
-         ++ destruct g1; try done.
-            move: (valid_fun_not_le_fun_nil Ng_g Vg LEf). done.
-      -- destruct g; try done.
-         destruct (~~ is_nil g1) eqn:Ng_g1.
-         ++ have Vw1i: valid w1i by eapply (valid_app Vg1 Vui A1i).
-            move: (H2 _ _ bot Inf (app_nil_eq _)) => Hwt.
-            eapply Hwt. eapply wt_bot; eauto. 
-            instantiate (2:= max i0 i). instantiate (1:= (S (max i0 i))).
-            eapply wt_tuniv. lia.
-            eapply le_bot. 
-            eauto.
-         ++ destruct g1; try done.
-            rewrite app_nil_eq in A1i. inversion A1i. subst.
-            move: (H1 _ _ bot Inf (app_nil_eq _)) => Hwt.
-            exact Hwt.
-Admitted.
-*)
-
-(*
-Lemma wt_WT u a : wt u a -> WT u a.
-induction 1.
-all: split; [ move => i0 WTa b LE WTb 
-            | move=> v w Wtv LUB;
-              inversion LUB; subst; try done;
-              destruct v; try done;
-              try solve [cbn in LUB; inversion LUB; 
-                  subst; econstructor; eauto]
-            | try (move=> w b f EQ1 EQ2; inversion EQ1; subst)
-  ].
-(* bot *)
-- eapply wt_bot; eauto.
-(* tuniv *)
-- apply le_tuniv_inv in LE. subst. 
-  eapply wt_tuniv; eauto.
-- cbn in LUB.
-  destruct (i=?n) eqn:EQ. rewrite Nat.eqb_eq in EQ. subst.
-  inversion LUB. done. inversion LUB.
-(* tnat *)
-- apply le_tuniv_inv in LE. subst.
-  eapply wt_tnat; eauto.
-(* zero *)
-- apply le_tnat_inv in LE. subst.
-  eapply wt_zero; eauto.
-(* succ *)
-- eapply le_tnat_inv in LE. subst.
-  eapply wt_succ; eauto.
-- cbn in LUB. destruct (lub u v) eqn:EQ; try done. inversion LUB.
-  inversion Wtv. subst.
-  eapply WT_lub in EQ; eauto. eapply wt_succ; eauto. 
-(* tpi *)
-- apply le_tuniv_inv in LE. subst.    
-    eapply wt_tpi; eauto.
-(* tpi - lub *)
-- destruct (compatible_fun g l) eqn:C1; try done.
-  destruct (lub a v) eqn:L1; try done.
-  inversion H6. clear H6.
-  (* e = lub a v *)
-  inversion Wtv; subst. clear Wtv.
-  have Va : valid a. eauto with valid.
-  have Vv : valid v. eauto with valid.
-  have Ve : valid e. eauto with valid.
-  eapply wt_tpi; eauto.
-  + move=> ui vi InApp.
-    destruct (in_app_or _ _ _ InApp) as [Ing|Inl].
-      ++ (* tuple is in the original list *) 
-         specialize (H0 _ _ Ing). 
-         eapply WT_le; eauto.
-         eapply le_lub_left; eauto.
-         eapply lub_compatible; eauto.
-         eapply WT_lub; eauto.
-      ++ (* tuple is in l -- can't use IH for WT_le *)
-        move: (H9 _ _ Inl) => WTui.
-        eapply WT_le; eauto.
-        eapply le_lub_right; eauto.
-        eapply lub_compatible; eauto.
-        eapply WT_lub; eauto.
-    + move=> ui vi InApp.
-      destruct (in_app_or _ _ _ InApp) as [Ing|Inl]; eauto.
-    + apply /andP. fold valid (valid_fun (g ++ l)).
-      split. eauto.
-      move: H3 => /andP [_ Vg]. fold valid (valid_fun g) in Vg.
-      move: H11 => /andP [_ Vl]. fold valid (valid_fun l) in Vl.
-      eapply valid_append; eauto.
-*)
+(* wt is monotone *)
 
 (*
 Lemma 2 
@@ -516,46 +245,34 @@ Proof.
   apply /andP. split; auto.
 Qed. *)
 
-Lemma compatible_app_inv f g u v :
-  valid_fun f -> 
-  valid_fun g -> 
-  valid u ->
-  compatible_fun f g ->
-  app (f ++ g) u = Some v -> 
-  { vf & { vg &  app f u = Some vf /\ app g u = Some vg /\ lub vf vg = Some v}}.
-Proof.
-  move=> Vf Vg Vu Cfg APPu.
-  destruct (valid_app_exists Vf Vu) as [vf [APPf Vvf]].
-  destruct (valid_app_exists Vg Vu) as [vg [APPg Vvg]].
-  move: (app_append_eq Cfg APPf APPg) => EQ.
-  exists vf. exists vg.
-  repeat split; eauto.
-  rewrite APPu in EQ. done.
-Qed.
 
 (* - If u : a, v : a, and u and v are compatible, then lub u v : a *)
-Fixpoint wt_lub u a (h: wt u a) {struct h}
+Lemma wt_lub u a (h: wt u a) 
   : forall v w, wt v a -> lub u v = Some w -> wt w a.
 Proof.
-  - dependent destruction h.
+  induction h.
   all: move=> v w1 Wtv LUB.
   all: inversion LUB; subst; try done.
   all: destruct v; try done.
   all: try solve [cbn in LUB; inversion LUB;
                   subst; econstructor; eauto].
-  + destruct (lub u v) eqn:EQ; try done.
-    cbn in H0. inversion H0. subst.
+  + (* u = succ u, v = succ v *)
+    destruct (lub u v) eqn:EQ; try done.
+    match goal with [H0 : option_map _ (Some _) = _ |- _] =>
+    cbn in H0; inversion H0 end. 
+    subst.
     inversion Wtv; subst.
     eapply wt_succ; eauto.
   + (* u = tpi a g, v=tpi v l *)
     destruct (compatible_fun g l) eqn:C1; try done.
     destruct (lub a v) eqn:L1; try done.
-    inversion H0. clear H0. subst.
+    match goal with [H0 : option_map _ (Some _) = _ |- _] =>
+    cbn in H0; inversion H0; clear H0 end. 
     (* e = lub a v *)
     clear LUB.
     inversion Wtv; subst. clear Wtv.
     eapply wt_tpi.
-    ++ eapply wt_lub in L1; eauto. 
+    ++ eapply IHh in L1; eauto. 
     ++ move=> ui vi Vui APP NB.
        have Vg: valid_fun g. eauto with valid.
        have Vl: valid_fun l. eauto with valid.
@@ -565,15 +282,16 @@ Proof.
        destruct (is_bot v2) eqn:N2.
        { destruct v1; destruct v2; try done. cbn in h3. 
          inversion h3. subst. done. }
-       { have Nb2: ~ is_bot v2. rewrite N2. done.
-         specialize (H2 ui v2 Vui APP2 Nb2).
+       { have Nb2: ~ is_bot v2. 
+         rewrite N2. done.
+         specialize (H5 ui v2 Vui APP2 Nb2).
          eapply wt_le; eauto. 
          eapply le_lub_right; eauto.
          eapply lub_compatible; eauto.
          eauto with valid.
          eauto with valid. } 
        { have Nb1 : ~ is_bot v1. rewrite N1. done. 
-         specialize (w ui v1 Vui APP1 Nb1).
+         specialize (w0 ui v1 Vui APP1 Nb1).
          eapply wt_le; eauto.
          eapply le_lub_left; eauto.
          eapply lub_compatible; eauto.
@@ -584,26 +302,24 @@ Proof.
        have Vl: valid_fun l. eauto with valid.
        move: (compatible_app_inv Vg Vl Vui C1 APP) => 
              [v1 [v2 [APP1 [APP2 h3]]]].
-       have WT1: wt v1 tuniv.
-       { destruct (is_bot v1) eqn:N1. 
-         - destruct v1; try done. eapply wt_bot. eapply wt_tuniv.
-         - have Nb1 : ~ is_bot v1. rewrite N1. done. 
-           exact (w0 ui v1 Vui APP1 Nb1).
-       } 
-       have WT2: wt v2 tuniv.
-       { destruct (is_bot v2) eqn:N2.
-         - destruct v2; try done. eapply wt_bot. eapply wt_tuniv.
-         - have Nb2: ~ is_bot v2. rewrite N2. done.
-           exact (H3 ui v2 Vui APP2 Nb2).
-       }
-       eapply (wt_lub _ _ WT1 _ _ WT2 h3); eauto.
+       destruct (is_bot v1) eqn:N1. 
+       { destruct v1; try done. inversion h3. subst.  eauto. } 
+       destruct (is_bot v2) eqn:N2.
+       { destruct v2; try done. rewrite lub_bot_r in h3. inversion h3. subst. eauto. }
+       have Nb1 : ~ is_bot v1. rewrite N1. done. 
+       have Nb2: ~ is_bot v2. rewrite N2. done.
+       have WT1: wt v1 tuniv.  { exact (w0 ui v1 Vui APP1 Nb1). } 
+       have WT2: wt v2 tuniv.  { exact (H6 ui v2 Vui APP2 Nb2). } 
+       eapply (H0 ui v1 Vui APP1 Nb1 v2 vi WT2 h3) .
     ++ eapply valid_tpi_intro.
        eapply (@valid_lub a v); eauto with valid.
        eapply valid_append; eauto with valid.
   + (* u = abs f, v=abs l *)
+    rename H into IHdom.
+    rename H0 into IHrng.
     cbn in LUB.
     destruct (compatible_fun f l) eqn:C1; try done.
-    inversion LUB; subst w1; clear LUB. clear H0.
+    inversion LUB; subst w1; clear LUB.
     inversion Wtv. subst. clear Wtv.
     eapply wt_abs.
     ++ move=> u v Vu APP NB.
@@ -616,47 +332,44 @@ Proof.
        { destruct v1; destruct v2; try done. cbn in h3. 
          inversion h3. subst. done. }
        { have Nb2: ~ is_bot v2. rewrite N2. done.
-         specialize (H2 u v2 Vu APP2 Nb2).
-         done. } 
+         eapply H3; eauto. }
        { have Nb1 : ~ is_bot v1. rewrite N1. done. 
-         specialize (w u v1 Vu APP1 Nb1).
-         done. } 
-    ++ move=> u v t Vu APP NB APPg.
+         eapply (w u v1 Vu APP1 Nb1); eauto.
+       } 
+    ++ (* wt rng for (f ++ l) *)
+       move=> u v t Vu APP NB APPg.
        have Vf: valid_fun f. eauto with valid.
        have Vl: valid_fun l. eauto with valid.
        move: (compatible_app_inv Vf Vl Vu C1 APP) => 
              [v1 [v2 [APP1 [APP2 h3]]]].
+       have WTt: wt t tuniv.
+       { destruct (is_bot t) eqn: NT.
+         destruct t; try done. eapply wt_bot. eapply wt_tuniv.
+         have Nb1:~ is_bot t. rewrite NT. done.
+         eapply wt_tpi_inv2; eauto. } 
        have WT1: wt v1 t.
        { destruct (is_bot v1) eqn:N1. 
          - destruct v1; try done. 
-           inversion H5.
-           destruct (is_bot t) eqn:NT. 
-           -- destruct t; try done.
-              eapply wt_bot. eapply wt_bot. eapply wt_tuniv.
-           -- eapply wt_bot. eapply (H7 u t Vu APPg).
-              rewrite NT. done.
+           eapply wt_bot; eauto.
          - have Nb1 : ~ is_bot v1. rewrite N1. done. 
            exact (w0 u v1 t Vu APP1 Nb1 APPg).
        } 
        have WT2: wt v2 t.
        { destruct (is_bot v2) eqn:N2.
-         - destruct v2; try done. eapply wt_bot. 
-           inversion H5.
-           destruct (is_bot t) eqn:NT. 
-           -- destruct t; try done.
-              eapply wt_bot. eapply wt_tuniv.
-           -- eapply (H7 u t Vu APPg).
-              rewrite NT. done.           
+         - destruct v2; try done. eapply wt_bot; eauto. 
          - have Nb2: ~ is_bot v2. rewrite N2. done.
-           exact (H3 u v2 t Vu APP2 Nb2 APPg).
+           exact (H4 u v2 t Vu APP2 Nb2 APPg).
        }
-       eapply (wt_lub _ _ WT1 _ _ WT2 h3); eauto.
+       destruct (is_bot v1) eqn:N1.
+       - destruct v1; try done. cbn in h3. inversion h3. subst. done.
+       - have Nb1: ~ (is_bot v1). rewrite N1. done.
+         eapply (IHrng u v1 t Vu APP1 Nb1 APPg v2 v WT2 h3).
     ++ cbn.
        apply /andP. split.
        eapply valid_append; eauto with valid.
        destruct f; try done.
     ++ done.
-Admitted. (* termination proof. *)
+Qed.
 
 
 (* Corollary 2 If w : Πaf and u : a, then w(u) : f (u). *)
@@ -737,352 +450,3 @@ Proof.
       inversion A1. subst r. done.
 Admitted.
 
-
-(*
-Lemma 3 If Πaf : Uk and f = (u1 → t1,...,un → tn), then ui : a and f (ui) : Uk. 
-
-This version is not the same as it doesn't say anything 
-intensional about f.
-
-*)
-
-(*
-Lemma lemma3_1 a f k : 
-  wt (tpi a f) (tuniv k) -> 
-  forall ui vi, In (ui,vi) f -> wt ui a.
-Proof.
-  intros.
-  inversion H. eauto.
-Qed.
-*)
-
-(*
-Lemma wt_instantiate a f k : 
-  wt (tpi a f) (tuniv k) -> 
-  forall ui w, wt ui a -> app f ui = Some w -> wt w (tuniv k).
-Proof.
-  induction f as [|[u v]f].
-  all: move=> WT; inversion WT; subst; clear WT.
-  all: move=> ui vi w. 
-  - rewrite app_nil_eq. move=> EQ. inversion EQ. subst.
-    eapply wt_bot; eauto.
-    admit.
-  - rewrite app_spec. cbn. rewrite <- app_spec.
-    destruct (compatible u ui && le u ui) eqn:EQ.
-    + move=> LUB. destruct (app f ui) eqn:APP; try done.
-      cbn [valid] in H5. fold (valid_fun ((u,v)::f)) in H5.
-      move: H5 => /andP [Va Vuf]; try done.
-      have WTv : wt v (tuniv k). 
-      { eapply H3; eauto. left. reflexivity. } 
-      have WT: wt (tpi a f) (tuniv k).
-      { destruct (~~ is_nil f) eqn:Nf.
-        - eapply wt_tpi; eauto.
-        move=> uj vj Infj. eapply H2; eauto. right; eauto.
-        move=> uj vj Infj. eapply H3; eauto. right; eauto.
-        apply /andP. fold valid. fold (valid_fun f).
-        split; auto. eauto with valid.
-      - destruct f; try done.
-        eapply wt_tpi; eauto; try done.
-        apply /andP. auto. 
-    } 
-    specialize (IHf WT).
-    eapply wt_lub in LUB; eauto.
-    + move=> APP.
-      eapply IHf; eauto.
-      eapply wt_tpi; eauto.
-      move=> uj vj Infj. eapply H2; eauto. right; eauto.
-      move=> uj vj Infj. eapply H3; eauto. right; eauto.
-      move: H5 => /andP [Va Vf]. fold valid in Va, Vf.
-      apply /andP. fold valid. split; auto.      
-      fold (valid_fun f).
-      eapply valid_fun_tail; eauto.
-Admitted.
-
-Lemma lemma3_2 a f k : 
-  wt (tpi a f) (tuniv k) -> 
-  forall ui vi w, In (ui,vi) f -> app f ui = Some w -> wt w (tuniv k).
-Proof.
-  intros.
-  inversion H. subst.
-  eapply wt_instantiate; eauto.
-Qed.
-*)
-
-(*
-Lemma 4:
-
-If w : Πaf and w = (u1 → t1,...,un → tn), then ui : a
-and w(ui) : f (ui).
-*)
-
-(*
-Lemma lemma4_1 w a f :
-  wt (abs w) (tpi a f) ->
-  forall ui vi, In (ui, vi) w -> wt ui a.
-Proof.
-  move=> WT ui vi In.
-  inversion WT as [| | | | | |aX wX fX j HuiAll HviAll Vabs WTtpi]; subst.
-  have Vw : valid_fun w. eauto with valid.
-  have Vui : valid ui.
-  { move: (valid_fun_subterms_prop Vw In) => [Vu _]. done. }
-  have Vtpi : valid (tpi a f). eauto with valid.
-  destruct (app_tpi_exists Vtpi Vui) as [t [At Vt]].
-  eapply HuiAll; eauto.
-Qed.
-
-Lemma lemma4_2 w a f :
-  wt (abs w) (tpi a f) ->
-  forall ui vi r t, In (ui, vi) w ->
-           app w ui = Some r -> app f ui = Some t -> wt r t.
-Proof.
-  move=> WT ui vi r t In Aw Af.
-  eapply wt_app; eauto.
-  eapply lemma4_1; eauto.
-Qed.
-*)
-
-(*
-Lemma 5 If w : Π b f and b <= a, then for any u : a there exists v : b such that v <= u and w(u) = w(v).
-
-Proof We write w = (u1 → l1,...,un → ln) with ui : b and 
-   li : f (ui). We then
-have w(u) = w(v) 
-   with v = ∨{ui | ui <= u} and v : b by Lemma 2.
-
-*)
-
-(*
-(* Stronger form: for any x with le v x and le x u, app w u = app w x. *)
-Lemma app_down_strong w b f :
-  wt (abs w) (tpi b f) -> forall u a,
-      le b a ->
-      wt u a ->
-      { v & (wt v b) * ( ( le v u) * 
-        (forall x, valid x -> le v x -> le x u -> app w u = app w x)) }.
-Proof.
-  induction w as [|[ui vi] w'].
-  - move=> WT. inversion WT. done.
-  - move=> WT u a LE WTu.
-    have Vu : valid u by eauto with valid.
-    have Vtpi : valid (tpi b f) by eauto with valid.
-    have Vabs : valid (abs ((ui,vi) :: w')) by eauto with valid.
-    have Vb : valid b.
-    { cbn in Vtpi. move: Vtpi => /andP [? _]. done. }
-    move: Vabs => /andP [Vw _]. fold (valid_fun ((ui,vi) :: w')) in Vw.
-    have Vui : valid ui by eapply key_valid; eauto using valid_fun_head.
-    have Vvi : valid vi by eapply val_valid; eauto using valid_fun_head.
-    have [wi [Awi Vwi]] : exists wi, app f ui = Some wi /\ valid wi
-      by eapply app_tpi_exists; eauto.
-    inversion WT as [| | | | | |aX wX fX j Hui2 Hvi2 VabsX VtpiX]; subst.
-    have WTui_b : wt ui b. admit.
-    destruct (~~ is_nil w') eqn:Nw.
-    + (* w' non-nil: use IH *)
-      have WTw' : wt (abs w') (tpi b f) by eapply wt_abs_pred; eauto.
-      destruct (IHw' WTw' u a LE WTu) as [v' [WTv' [LEv' IH2]]].
-      have Vv' : valid v' by eapply wt_valid_tm; eauto.
-      destruct (le ui u) eqn:LEui.
-      * (* le ui u = true *)
-        have Cui : compatible ui u by eapply le_valid_compatible; eauto using le_refl.
-        have Cuiv' : compatible ui v'.
-        { apply compatible_sym. eapply comp_down; eauto.
-          apply compatible_sym; eauto. }
-        destruct (compatible_lub_exists Cuiv') as [v_new EQv].
-        have Vv_new : valid v_new. { eapply (valid_lub Vui Vv' EQv). }
-        have LE_uivn : le ui v_new. { eapply (le_lub_left Cuiv' EQv Vui Vv'). }
-        have LE_vvn : le v' v_new. { eapply (le_lub_right Cuiv' EQv Vui Vv'). }
-        have LE_vnu : le v_new u. { eapply (@le_sup_lub ui v' v_new u LEui LEv' EQv). }
-        have WT_vnew : wt v_new b. { eapply wt_lub; [exact WTui_b | exact WTv' | exact EQv]. }
-        exists v_new. split; [|split]; eauto.
-        move=> x Vx LE_vnx LE_xu.
-        have LE_uix : le ui x by eapply le_trans with (v := v_new); eauto.
-        have LE_v'x : le v' x by eapply le_trans with (v := v_new); eauto.
-        have Cuix : compatible ui x by eapply le_valid_compatible; eauto.
-        have App_eq : app w' u = app w' x by apply IH2; eauto.
-        rewrite app_spec. cbn. rewrite <- app_spec.
-        rewrite Cui LEui Cuix LE_uix /=.
-        rewrite App_eq. reflexivity.
-      * (* le ui u = false *)
-        exists v'. split; [|split]; eauto.
-        move=> x Vx LE_v'x LE_xu.
-        have LE_uix : le ui x = false.
-        { destruct (le ui x) eqn:E; try reflexivity.
-          have Luiu : le ui u by eapply le_trans with (v := x); eauto.
-          rewrite LEui in Luiu. done. }
-        have App_eq : app w' u = app w' x by apply IH2; eauto.
-        rewrite app_spec. cbn. rewrite <- app_spec.
-        rewrite LEui LE_uix !Bool.andb_false_r /=.
-        exact App_eq.
-    + (* w' nil *)
-      destruct w'; try done.
-      destruct (le ui u) eqn:LEui.
-      * (* le ui u = true *)
-        have Cui : compatible ui u by eapply le_valid_compatible; eauto.
-        exists ui. split; [|split]; eauto.
-        move=> x Vx LE_uix LE_xu.
-        have Cuix : compatible ui x by eapply le_valid_compatible; eauto.
-        rewrite app_spec. cbn.
-        rewrite Cui LEui Cuix LE_uix /=.
-        rewrite !lub_bot_r. reflexivity.
-      * (* le ui u = false *)
-        exists bot. split; [|split].
-        -- eapply wt_bot; eauto. admit.
-        -- eapply le_bot.
-        -- move=> x Vx LE_botx LE_xu.
-           have LE_uix : le ui x = false.
-           { destruct (le ui x) eqn:E; try reflexivity.
-             have Luiu : le ui u by eapply le_trans with (v := x); eauto.
-             rewrite LEui in Luiu. done. }
-           rewrite app_spec. cbn.
-           rewrite LEui LE_uix !Bool.andb_false_r /=.
-           reflexivity.
-Admitted.
-
-Lemma app_down w b f :
-  wt (abs w) (tpi b f) -> forall u a,
-      le b a ->
-      wt u a -> exists v, wt v b /\ le v u /\ app w u = app w v.
-Proof.
-  move=> WT u a LE WTu.
-  destruct (app_down_strong WT LE WTu) as [v [WTv [LEv HStr]]].
-  have Vv : valid v by eapply wt_valid_tm; eauto.
-  exists v. split; [|split]; eauto.
-  eapply HStr; eauto. eapply le_refl; eauto.
-Qed.
-*)
-
-(* NOT TRUE *)
-Lemma wt_compatible:
-  forall ui ai, wt ui ai -> forall uj aj, wt uj aj -> 
-                               compatible ai aj -> 
-                               compatible ui uj.
-Proof.
-  move=> ui ai h.
-  induction h.
-  all: move=> ui ai WTi CC.
-  all: try solve [destruct ui; done].
-  all: destruct ai; try done.
-  all: try match goal with [ H : wt _ bot |- _ ] => inversion WTi; subst; done end.
-  all: inversion CC; subst; clear CC.
-Abort.
-
-(* ------------------------------------------------------------- *)
-(*
-Inductive is_type : elt -> Prop :=
-  | is_bot : is_type bot
-  | is_tuniv i : is_type (tuniv i)
-  | is_tnat : is_type tnat
-  | is_tpi a f :
-    valid (tpi a f) ->
-    is_type a ->
-    (forall u v, In (u,v) f -> wt u a) ->
-    (forall u v, In (u,v) f -> is_type v) ->
-    is_type (tpi a f).
-
-Lemma is_type_valid a : is_type a -> valid a.
-Proof.
-  induction 1; cbn; auto.
-Qed.
-
-Hint Resolve is_type_valid : valid.
-
-
-(* 
-If a : Uj , then a type. 
-If a type, b type, and a,b are compatible, then a ∨ b type. 
-If Π a (u1 → t1,...,un → tn) type and u1 → t1,...,un → tn is a
-minimal description, then ui : a and ti type.
-*)
-
-Lemma wt_is_type a i :
-  wt a (tuniv i) -> is_type a.
-Proof.
-  move=> h.
-  remember (tuniv i) as t eqn:Ht.
-  move: i Ht.
-  induction h; move=> k Heq; try discriminate.
-  - constructor.
-  - constructor.
-  - constructor.
-  - inversion Heq; subst j.
-    apply is_tpi.
-    + eauto.
-    + eauto.
-    + eauto.
-    + eauto.
-Qed.
-
-Lemma is_type_lub a b :
-  is_type a -> is_type b -> forall c, lub a b = Some c -> is_type c.
-Proof.
-  move=> Ta. move: b.
-  induction Ta as [ | i | | a0 f0 Va Ta0 IHa0 Hwt_f0 Hist_f0 IH_f0].
-  - move=> b Tb c L. cbn in L. inversion L; subst. exact Tb.
-  - move=> b Tb c L.
-    inversion Tb; subst; cbn in L; try discriminate.
-    + inversion L; subst. constructor.
-    + destruct (i =? i0) eqn:E; try discriminate.
-      inversion L; subst. constructor.
-  - move=> b Tb c L.
-    inversion Tb; subst; cbn in L; try discriminate.
-    + inversion L; subst. constructor.
-    + inversion L; subst. constructor.
-  - move=> b Tb c L.
-    inversion Tb as [| | | a1 f1 Va1_tpi Ta1 Hwt_f1 Hist_f1];
-      subst; cbn in L; try discriminate.
-    + inversion L; subst. eapply is_tpi; eauto.
-    + destruct (compatible_fun f0 f1) eqn:CF; try discriminate.
-      destruct (lub a0 a1) eqn:La; try discriminate.
-      cbn in L. inversion L; subst c; clear L.
-      have Va0 : valid a0 by eauto using is_type_valid.
-      have Va1 : valid a1 by eauto using is_type_valid.
-      have Ca : compatible a0 a1 by eapply lub_compatible; eauto.
-      have Ve : valid e by exact: (valid_lub Va0 Va1 La).
-      have LEae : le a0 e by exact: (le_lub_left Ca La Va0 Va1).
-      have LEbe : le a1 e by exact: (le_lub_right Ca La Va0 Va1).
-      have Te : is_type e by eapply IHa0; eauto.
-      have Vres : valid (tpi e (f0 ++ f1)).
-      { cbn. apply /andP. split; auto.
-        cbn in Va, Va1_tpi.
-        move: Va => /andP [Va Vf0].
-        move: Va1_tpi => /andP [_ Vf1].
-        eapply valid_append; eauto.
-      }         
-      eapply is_tpi; eauto.
-      * move=> u v Inv. apply in_app_or in Inv. destruct Inv as [Inv|Inv].
-        -- eapply wt_le; eauto. admit. admit.
-        -- eapply wt_le; eauto. admit. admit.
-      * move=> u v Inv. apply in_app_or in Inv. destruct Inv as [Inv|Inv].
-        -- eapply Hist_f0; eauto.
-        -- eapply Hist_f1; eauto.
-Admitted.
-
-Lemma is_type_dom a f :
-  is_type (tpi a f) -> is_type a.
-Proof.
-  move=> H. inversion H. done.
-Qed.
-
-Lemma is_type_cod a f :
-  is_type (tpi a f) -> forall ui w, wt ui a -> app f ui = Some w -> is_type w.
-Proof.
-  induction f as [|[u v] f' IHf'].
-  - move=> _ ui w _ A.
-    rewrite app_nil_eq in A. inversion A; subst. constructor.
-  - move=> Ttpi ui w Wtui A.
-    inversion Ttpi as [| | |a2 f2 Vtpi Ta Hwt Hist]; subst.
-    have Tf' : is_type (tpi a f').
-    { have [Va Vu] := valid_tpi_inv Vtpi.
-      have Vtf' : valid (tpi a f').
-      { apply valid_tpi_intro; [exact Va|].
-        eauto with valid. }
-      apply is_tpi; auto;
-        move=> u' v' In'; [eapply Hwt|eapply Hist]; right; eauto. }
-    rewrite app_cons_eq in A.
-    destruct (compatible u ui && le u ui) eqn:E.
-    + destruct (app f' ui) as [t|] eqn:Afp; try discriminate.
-      have Tv : is_type v by eapply Hist; left; reflexivity.
-      have Tt : is_type t by eapply IHf'; eauto.
-      eapply is_type_lub; [exact Tv|exact Tt|exact A].
-    + eapply IHf'; eauto.
-Qed.
-*)
